refactor

src/drf/AbortProp.v
@@ -40,6 +40,604 @@ Require Import PFConsistent.
 Set Implicit Arguments.
 
 
+Section CANCEL.
+
+  Definition no_reserves (proms: Memory.t): Prop :=
+    forall loc to from msg (GET: Memory.get loc to proms = Some (from, msg)),
+      msg <> Message.reserve.
+
+  Inductive only_reserves (proms: Memory.t): Prop :=
+  | only_reserves_intro
+      (RESERVES: forall loc to from msg (GET: Memory.get loc to proms = Some (from, msg)),
+          msg = Message.reserve)
+      (FINITE: Memory.finite proms)
+  .
+
+  Lemma reserves_cancelable lang st vw proms0 sc mem0
+        (FINITE: Memory.finite proms0)
+        (MLE: Memory.le proms0 mem0)
+    :
+      exists proms1 mem1,
+        (<<STEPS: rtc (tau (@pred_step is_cancel lang))
+                      (Thread.mk lang st (Local.mk vw proms0) sc mem0)
+                      (Thread.mk lang st (Local.mk vw proms1) sc mem1)>>) /\
+        (<<NORESERVES: no_reserves proms1>>).
+  Proof.
+    assert (exists dom,
+               (<<COMPLETE: forall loc to,
+                   (exists from, (<<GET: Memory.get loc to proms0 = Some (from, Message.reserve)>>))
+                   <-> (<<IN: List.In (loc, to) dom>>)>>)).
+    { unfold Memory.finite in *. des.
+      generalize (list_filter_exists (fun locto =>
+                                        match locto with
+                                        | (loc, to) =>
+                                          exists from, Memory.get loc to proms0 = Some (from, Message.reserve)
+                                        end) dom).
+      i. des. exists l'. split; i.
+      - eapply COMPLETE. des. esplits; eauto.
+      - eapply COMPLETE in H. des. esplits; eauto. }
+    des. ginduction dom; ss; i.
+    - exists proms0, mem0. esplits; eauto.
+      ii. clarify. eapply COMPLETE. eauto.
+    - destruct a as [loc to].
+      exploit (proj2 (COMPLETE loc to)); eauto. i. des.
+      destruct (classic (List.In (loc, to) dom)).
+      { exploit IHdom; eauto. i. split; i.
+        - des. exploit (proj1 (COMPLETE loc0 to0)); eauto.
+          i. des; clarify.
+        - exploit (proj2 (COMPLETE loc0 to0)); eauto. }
+      exploit Memory.remove_exists; eauto.
+      intros [prom1 REMOVE0].
+      exploit Memory.remove_exists.
+      { eapply MLE. eapply GET. }
+      intros [mem1 REMOVE1]. hexploit IHdom.
+      * instantiate (1:=prom1).
+        eapply Memory.remove_finite; eauto.
+      * instantiate (1:=mem1).
+        ii. erewrite Memory.remove_o in LHS; eauto. des_ifs.
+        eapply MLE in LHS. erewrite Memory.remove_o; eauto. des_ifs.
+        ss. des; clarify.
+      * i. split; i.
+        { des. erewrite Memory.remove_o in GET0; eauto. des_ifs.
+          exploit (proj1 (COMPLETE loc0 to0)); eauto. i. des; clarify. }
+        { exploit (proj2 (COMPLETE loc0 to0)); eauto. i. des; clarify.
+          exists from0. erewrite Memory.remove_o; eauto. des_ifs.
+          ss. des; clarify. }
+      * i. des. exists proms1, mem2. split; eauto.
+        econs 2.
+        { econs.
+          - instantiate (2:=ThreadEvent.promise loc from to Message.reserve Memory.op_kind_cancel).
+            econs; ss. econs. econs 1. econs; ss.
+            econs; ss. econs; eauto.
+          - eauto. }
+        { eauto. }
+  Qed.
+
+  Lemma promise_not_cacncel_reserves_same prom0 mem0 loc from to msg prom1 mem1 kind
+        (PROM: Memory.promise prom0 mem0 loc from to msg prom1 mem1 kind)
+        (NOTCANCEL: kind <> Memory.op_kind_cancel)
+        loc0 to0 from0
+        (GET: Memory.get loc0 to0 prom0 = Some (from0, Message.reserve))
+    :
+      exists from1,
+        Memory.get loc0 to0 prom1 = Some (from1, Message.reserve).
+  Proof.
+    inv PROM.
+    - eapply Memory.add_get1 in GET; eauto.
+    - des. clarify. erewrite Memory.split_o; eauto.
+      dup PROMISES. eapply Memory.split_get0 in PROMISES0.
+      eapply split_succeed_wf in PROMISES. des. des_ifs.
+      + ss. des. clarify.
+      + ss. guardH o. des. clarify.
+        esplits; eauto.
+      + esplits; eauto.
+    - des. clarify. erewrite Memory.lower_o; eauto. des_ifs.
+      + ss. des. clarify.
+        eapply lower_succeed_wf in PROMISES. des. clarify.
+      + esplits; eauto.
+    - clarify.
+  Qed.
+
+  Lemma remove_not_cacncel_reserves_same prom0 loc from to val released prom1
+        (REMOVE: Memory.remove prom0 loc from to (Message.full val released) prom1)
+        loc0 to0 from0
+        (GET: Memory.get loc0 to0 prom0 = Some (from0, Message.reserve))
+    :
+      exists from1,
+        Memory.get loc0 to0 prom1 = Some (from1, Message.reserve).
+  Proof.
+    dup REMOVE. eapply Memory.remove_get0 in REMOVE. des.
+    eapply Memory.remove_o in REMOVE0.
+    instantiate (1:=to0) in REMOVE0.
+    instantiate (1:=loc0) in REMOVE0. des_ifs.
+    - ss. des. clarify.
+    - esplits. etrans; eauto.
+  Qed.
+
+  Lemma step_not_cancel_reserves_same P lang e th0 th1
+        (STEPS: (@pred_step P lang) e th0 th1)
+        (PRED: P <1= (promise_free /1\ (fun e => ~ is_cancel e)))
+        loc to from
+        (GET: Memory.get loc to th0.(Thread.local).(Local.promises) = Some (from, Message.reserve))
+    :
+      exists from',
+        Memory.get loc to th1.(Thread.local).(Local.promises) = Some (from', Message.reserve).
+  Proof.
+    inv STEPS. eapply PRED in SAT. inv STEP. inv STEP0.
+    - inv STEP. des. ss. inv LOCAL.
+      eapply promise_not_cacncel_reserves_same; eauto.
+      ii. clarify.
+    - inv STEP. inv LOCAL; ss.
+      + esplits; eauto.
+      + inv LOCAL0. esplits; eauto.
+      + inv LOCAL0. inv WRITE. ss.
+        eapply promise_not_cacncel_reserves_same in GET; cycle 1; eauto.
+        { ii. clarify. inv PROMISE. clarify. } des.
+        eapply remove_not_cacncel_reserves_same in GET; cycle 1; eauto.
+      + inv LOCAL2. inv WRITE. ss. inv LOCAL1. ss.
+        eapply promise_not_cacncel_reserves_same in GET; cycle 1; eauto.
+        { ii. clarify. inv PROMISE. clarify. } des.
+        eapply remove_not_cacncel_reserves_same in GET; cycle 1; eauto.
+      + inv LOCAL0. esplits; eauto.
+      + inv LOCAL0. esplits; eauto.
+      + inv LOCAL0. esplits; eauto.
+  Qed.
+
+  Lemma steps_not_cancel_reserves_same P lang th0 th1
+        (STEPS: rtc (tau (@pred_step P lang)) th0 th1)
+        (PRED: P <1= (promise_free /1\ (fun e => ~ is_cancel e)))
+        loc to from
+        (GET: Memory.get loc to th0.(Thread.local).(Local.promises) = Some (from, Message.reserve))
+    :
+      exists from',
+        Memory.get loc to th1.(Thread.local).(Local.promises) = Some (from', Message.reserve).
+  Proof.
+    ginduction STEPS; i.
+    - esplits; eauto.
+    - inv H. exploit step_not_cancel_reserves_same; eauto. i. des.
+      exploit IHSTEPS; eauto.
+  Qed.
+
+  Lemma cancel_promises_decrease P lang e th0 th1
+        (STEP: (@pred_step P lang) e th0 th1)
+        (PRED: P <1= is_cancel)
+    :
+      Memory.le th1.(Thread.local).(Local.promises) th0.(Thread.local).(Local.promises).
+  Proof.
+    inv STEP. eapply PRED in SAT. unfold is_cancel in SAT. des_ifs.
+    inv STEP0. inv STEP; inv STEP0; ss.
+    - inv LOCAL. inv PROMISE; ss.
+      ii. erewrite Memory.remove_o in LHS; eauto. des_ifs.
+    - inv LOCAL.
+  Qed.
+
+  Lemma cancels_promises_decrease P lang th0 th1
+        (STEP: rtc (tau (@pred_step P lang)) th0 th1)
+        (PRED: P <1= is_cancel)
+    :
+      Memory.le th1.(Thread.local).(Local.promises) th0.(Thread.local).(Local.promises).
+  Proof.
+    ginduction STEP.
+    - refl.
+    - etrans; eauto. inv H.
+      eapply cancel_promises_decrease; eauto.
+  Qed.
+
+End CANCEL.
+
+Section CAP.
+
+  Definition caps (mem0 prom : Memory.t) (l : Loc.t) (t from : Time.t) (msg : Message.t) :=
+    forall mem1 (CAP: Memory.cap prom mem0 mem1),
+      (<<GET0: Memory.get l t mem0 = None>>) /\
+      (<<GET1: Memory.get l t mem1 = Some (from, msg)>>).
+
+  Definition caps_loc (mem0 prom : Memory.t) (l : Loc.t) (t : Time.t): Prop :=
+    exists from msg, (<<CAPS: caps mem0 prom l t from msg>>).
+
+  Lemma caps_unchangable mem0 prom mem1
+        (MLE: Memory.le prom mem0)
+        (CAP: Memory.cap prom mem0 mem1)
+    :
+      caps mem0 prom <4= unchangable mem1 prom.
+  Proof.
+    i. exploit PR; eauto. i. des. inv CAP.
+    econs; eauto. ii. inv H.
+    destruct msg. eapply MLE in GET. clarify.
+  Qed.
+
+  Lemma caps_concrete_last mem0 prom mem1 tm l t from val released
+        (RESERVE: Memory.reserve_wf prom mem0)
+        (INHABITED: Memory.inhabited mem0)
+        (MAX: Memory.max_full_timemap mem0 tm)
+        (CAP: Memory.cap prom mem0 mem1)
+        (CAPS: caps mem0 prom l t from (Message.full val released))
+    :
+      from = Memory.max_ts l mem0.
+  Proof.
+    exploit CAPS; eauto. i. des. inv CAP.
+    exploit COMPLETE; eauto. i. des.
+    destruct (classic (Memory.max_ts l mem0 = from)); eauto. exfalso.
+    set (@cell_elements_least
+           (mem0 l)
+           (fun to => Time.lt from to)). des.
+    + assert (TLE: Time.le from from0).
+      { dup GET. eapply Memory.get_ts in GET. des; clarify.
+        { exfalso. eapply Time.lt_strorder.
+          eapply TimeFacts.lt_le_lt; eauto. eapply Time.bot_spec. }
+        exploit memory_get_from_mon.
+        - eapply x.
+        - eapply GET2.
+        - eauto.
+        - i. des; clarify. refl. }
+      destruct TLE.
+      * exploit MIDDLE; eauto.
+        econs.
+        { eapply x. }
+        { eapply GET. }
+        { eauto. }
+        { i. destruct (Memory.get l ts mem0) eqn: GET2; auto.
+          destruct p. exfalso. dup GET2. eapply LEAST in GET2; eauto.
+          eapply Memory.get_ts in GET. des; clarify.
+          - eapply Time.lt_strorder. eapply TimeFacts.lt_le_lt.
+            eapply SAT. eapply Time.bot_spec.
+          - eapply Time.lt_strorder. eapply TimeFacts.lt_le_lt.
+            eapply GET. etrans; eauto. }
+        { i. exploit memory_get_from_inj.
+          - eapply x1.
+          - eapply GET1.
+          - i. des; clarify. eapply Time.lt_strorder; eauto. }
+      * destruct H0.
+        exploit memory_get_from_inj.
+        { eapply GET1. }
+        { eapply SOUND. eapply GET. }
+        { i. des; clarify.
+          - unfold Memory.get in GET0. clarify.
+          - eapply Time.lt_strorder; eauto. }
+    + exploit Memory.max_ts_spec.
+      { eapply x. } i. des.
+      eapply EMPTY; eauto. destruct MAX0; clarify.
+      exfalso. eauto.
+  Qed.
+
+  Lemma caps_max_view mem0 prom mem1 tm l t from val released
+        (RESERVE: Memory.reserve_wf prom mem0)
+        (INHABITED: Memory.inhabited mem0)
+        (MAX: Memory.max_full_timemap mem0 tm)
+        (CAP: Memory.cap prom mem0 mem1)
+        (CAPS: caps mem0 prom l t from (Message.full val released))
+    :
+      (<<FROM: from = Memory.max_ts l mem0>>) /\
+      (<<RESERVE: Memory.latest_reserve l prom mem0>>) /\
+      (<<VAL: Memory.latest_val l mem0 val >>) /\
+      (<<RELEASED: released = Some (View.mk tm tm)>>) /\
+      (<<TO: t = Time.incr (Memory.max_ts l mem0)>>).
+  Proof.
+    exploit caps_concrete_last; eauto. i. clarify.
+    exploit CAPS; eauto. i. des. inv CAP.
+    exploit COMPLETE; eauto. i. des.
+    exploit Memory.latest_val_exists; eauto. i. des.
+    exploit BACK; eauto. i.
+    exploit memory_get_from_inj.
+    { eapply x1. }
+    { eapply GET1. } i. des; clarify.
+    - esplits; eauto.
+    - exfalso. eapply Time.lt_strorder. eapply TimeFacts.lt_le_lt.
+      + eapply Time.incr_spec.
+      + erewrite BOT0. eapply Time.bot_spec.
+    - erewrite INHABITED in GET0. clarify.
+  Qed.
+
+End CAP.
+
+Section PROMISEFREE.
+
+  Lemma promise_free_no_promise P lang (th0 th1: Thread.t lang) e
+        (NOPROMISE: th0.(Thread.local).(Local.promises) = Memory.bot)
+        (STEP: pred_step P e th0 th1)
+        (PRED: P <1= promise_free)
+  :
+    (<<STEP: pred_step P e th0 th1>>) /\
+    (<<NOPROMISE: th1.(Thread.local).(Local.promises) = Memory.bot>>).
+  Proof.
+    inv STEP. dup SAT. eapply PRED in SAT. inv STEP0. inv STEP.
+    - inv STEP0. inv LOCAL. inv PROMISE; ss; des; clarify.
+      + rewrite NOPROMISE in *.
+        eapply Memory.lower_get0 in PROMISES. des.
+        erewrite Memory.bot_get in *. clarify.
+      + rewrite NOPROMISE in *.
+        eapply Memory.remove_get0 in PROMISES. des.
+        erewrite Memory.bot_get in *. clarify.
+    - inv STEP0. inv LOCAL.
+      + ss. esplits; eauto. econs; eauto. econs; eauto.
+      + ss. esplits; eauto.
+        * econs; eauto. econs; eauto.
+        * inv LOCAL0. ss.
+      + ss. esplits; eauto.
+        * econs; eauto. econs; eauto.
+        * inv LOCAL0. rewrite NOPROMISE in *.
+          exploit memory_write_bot_add; eauto. i. clarify.
+          inv WRITE. inv PROMISE. ss.
+          symmetry. eapply MemoryMerge.MemoryMerge.add_remove; eauto.
+      + ss. esplits; eauto.
+        * econs; eauto. econs; eauto.
+        * inv LOCAL1. inv LOCAL2. rewrite NOPROMISE in *.
+          exploit memory_write_bot_add; eauto. i. clarify.
+          inv WRITE. inv PROMISE. ss.
+          symmetry. eapply MemoryMerge.MemoryMerge.add_remove; eauto.
+      + ss. esplits; eauto.
+        * econs; eauto. econs; eauto.
+        * inv LOCAL0. ss.
+      + ss. esplits; eauto.
+        * econs; eauto. econs; eauto.
+        * inv LOCAL0. ss.
+      + ss. esplits; eauto.
+        * econs; eauto. econs; eauto.
+  Qed.
+
+  Lemma write_promises_decrease prom0 mem0 loc from to val realeased prom1 mem1 kind
+        (WRITE: Memory.write prom0 mem0 loc from to val realeased prom1 mem1 kind)
+    :
+      concrete_promised prom1 <2= concrete_promised prom0.
+  Proof.
+    inv WRITE. inv PROMISE.
+    - exploit MemoryMerge.MemoryMerge.add_remove.
+      + eapply PROMISES.
+      + eapply REMOVE.
+      + i. clarify.
+    - ii. inv PR.
+      erewrite Memory.remove_o in GET; eauto. des_ifs.
+      erewrite Memory.split_o in GET; eauto. des_ifs.
+      + ss; des; clarify.
+      + ss. des; clarify. eapply Memory.split_get0 in PROMISES.
+        des. econs; eauto.
+      + eapply Memory.split_get0 in PROMISES.
+        guardH o. guardH o0. guardH o1. des. econs; eauto.
+    - ii. inv PR.
+      erewrite Memory.remove_o in GET; eauto. des_ifs.
+      erewrite Memory.lower_o in GET; eauto. des_ifs.
+      + ss; des; clarify.
+      + econs; eauto.
+    - clarify.
+  Qed.
+
+  Lemma pf_step_promises_decrease P lang e (th0 th1: Thread.t lang)
+        (STEP: (@pred_step P lang) e th0 th1)
+        (PRED: P <1= promise_free)
+    :
+      concrete_promised (th1.(Thread.local).(Local.promises)) <2=
+      concrete_promised (th0.(Thread.local).(Local.promises)).
+  Proof.
+    i. inv STEP. eapply PRED in SAT. inv STEP0. des. inv STEP.
+    - inv STEP0. ss. inv LOCAL. ss. inv PROMISE; clarify.
+      + inv PR. erewrite Memory.lower_o in GET; eauto. des_ifs.
+        * ss; des. clarify. eapply Memory.lower_get0 in PROMISES.
+          des. econs; eauto.
+        * econs; eauto.
+      + inv PR. erewrite Memory.remove_o in GET; eauto. des_ifs.
+        econs; eauto.
+    - inv STEP0. ss. inv LOCAL; eauto.
+      + inv LOCAL0. ss.
+      + inv LOCAL0. ss. eapply write_promises_decrease; eauto.
+      + inv LOCAL1. inv LOCAL2. ss. eapply write_promises_decrease; eauto.
+      + inv LOCAL0. ss.
+      + inv LOCAL0. ss.
+  Qed.
+
+  Lemma pf_step_rtc_promises_decrease P lang (th0 th1: Thread.t lang)
+        (STEP: rtc (tau (@pred_step P lang)) th0 th1)
+        (PRED: P <1= promise_free)
+    :
+      concrete_promised (th1.(Thread.local).(Local.promises)) <2=
+      concrete_promised (th0.(Thread.local).(Local.promises)).
+  Proof.
+    ginduction STEP; ss.
+    i. eapply IHSTEP in PR; eauto. inv H.
+    eapply pf_step_promises_decrease; eauto.
+  Qed.
+
+End PROMISEFREE.
+
+
+Section PFCONSISTENT.
+
+  Definition pf_consistent_strong lang (e0:Thread.t lang): Prop :=
+    forall mem1 sc1
+           (CAP: Memory.cap e0.(Thread.local).(Local.promises) e0.(Thread.memory) mem1),
+    exists e1,
+      (<<STEPS0: rtc (tau (@pred_step is_cancel lang)) (Thread.mk _ e0.(Thread.state) e0.(Thread.local) sc1 mem1) e1>>) /\
+      (<<NORESERVE: no_reserves e1.(Thread.local).(Local.promises)>>) /\
+      exists e2,
+        (<<STEPS1: rtc (tau (@pred_step ((promise_free /1\ (fun e => ~ is_cancel e) /1\ no_acq_read_msgs (caps_loc e0.(Thread.memory) e0.(Thread.local).(Local.promises))) /1\ no_sc) lang)) e1 e2>>) /\
+        ((<<FAILURE: Local.failure_step e2.(Thread.local)>>) \/
+         (<<PROMISES: e2.(Thread.local).(Local.promises) = Memory.bot>>)).
+
+  Lemma pf_consistent_pf_consistent_strong lang (th: Thread.t lang)
+        (WF: Local.wf th.(Thread.local) th.(Thread.memory))
+        (MEM: Memory.closed th.(Thread.memory))
+        (INHABITED: Memory.inhabited th.(Thread.memory))
+        (CONSISTENT: pf_consistent th)
+    :
+      pf_consistent_strong th.
+  Proof.
+    ii. exploit Memory.max_full_timemap_exists; eauto. intros MAX. des.
+    ii. exploit Memory.max_full_timemap_exists.
+    { eapply le_inhabited; eauto. eapply Memory.cap_le; eauto. refl. }
+    i. des. exploit CONSISTENT; eauto. i.
+
+    assert (exists e2,
+               (<<STEPS: rtc (tau (Thread.step true))
+                             (Thread.mk _ (Thread.state th) (Thread.local th)
+                                        tm0 mem1) e2 >>) /\
+               (<<NORESERVES: no_reserves e2.(Thread.local).(Local.promises)>>) /\
+               (__guard__ ((exists e3, (<< FAILURE: Thread.step true ThreadEvent.failure e2 e3 >>)) \/
+                           (<<PROMISES: Local.promises (Thread.local e2) = Memory.bot >>)))).
+    { des.
+      - exploit Thread.rtc_tau_step_future.
+        + eapply rtc_implies; [|apply STEPS].
+          i. inv PR. econs; eauto. econs; eauto.
+        + ss. eapply Local.cap_wf; eauto.
+        + ss. eapply Memory.max_full_timemap_closed; eauto.
+        + ss. eapply Memory.cap_closed; eauto.
+        + i. des.
+          destruct e2. destruct local. inv WF2. ss.
+          exploit reserves_cancelable; eauto. i. des.
+          esplits.
+          * etrans.
+            { eapply STEPS. }
+            { eapply rtc_implies; [|apply STEPS0].
+              i. inv PR. inv TSTEP. inv STEP.
+              unfold is_cancel in SAT. des_ifs.
+              inv STEP0; inv STEP.
+              - econs; eauto. econs; eauto. econs; eauto.
+              - inv LOCAL. }
+          * ss.
+          * left. inv FAILURE; inv STEP. inv LOCAL. inv LOCAL0.
+            exists (Thread.mk _ st2 (Local.mk tview proms1) sc2 mem0).
+            ss. econs 2. econs; eauto. econs; eauto. econs; eauto.
+            eapply cancels_promises_decrease in STEPS0; auto. ss.
+            ii. eapply CONSISTENT0; eauto.
+      - unguard. esplits; eauto. rewrite PROMISES. ii.
+        rewrite Memory.bot_get in GET. clarify. }
+
+    clear x. des.
+    eapply pf_step_promise_free_step_rtc in STEPS.
+    eapply pf_steps_cancels_not_cancels in STEPS; cycle 1.
+    { ss. eapply Local.cap_wf; eauto. }
+    { ss. eapply Memory.cap_closed; eauto. }
+    { ss. eapply Memory.max_full_timemap_closed; eauto. } des.
+
+    exploit Thread.rtc_tau_step_future.
+    { eapply thread_steps_pred_steps. eapply STEPS1. }
+    { ss. eapply Local.cap_wf; eauto. }
+    { ss. eapply Memory.max_full_timemap_closed; eauto. }
+    { ss. eapply Memory.cap_closed; eauto. }
+    i. des. ss.
+
+    destruct th1. exploit no_sc_any_sc_rtc; try apply STEPS1; ss.
+    { i. unfold is_cancel in PR. des_ifs. }
+    i. des. instantiate (1:=sc1) in STEP. clear STEPS1.
+
+    eexists. splits.
+    { eapply STEP. }
+    { ss. ii. clarify.
+      eapply steps_not_cancel_reserves_same in STEPS2; eauto.
+      unguard. des.
+      - eapply NORESERVES; eauto.
+      - rewrite PROMISES in *. erewrite Memory.bot_get in STEPS2. clarify. }
+
+    eapply hold_or_not with (Q := no_acq_read_msgs (caps_loc (Thread.memory th) (Local.promises (Thread.local th))) /1\ no_sc) in STEPS2. des.
+
+    - destruct e2. ss.
+      exploit no_sc_any_sc_rtc; try eapply HOLD; eauto.
+      { ss. i. des. auto. } i. des.
+      esplits.
+      + eapply pred_step_rtc_mon; try eapply STEP0.
+        i. ss. des. splits; eauto.
+      + ss. unguard. des.
+        * left. ss. inv FAILURE; inv STEP1. inv LOCAL. eauto.
+        * right. esplits; eauto.
+
+    - exploit Thread.rtc_tau_step_future.
+      { eapply thread_steps_pred_steps. eapply STEPS0. }
+      { ss. }
+      { ss. }
+      { ss. } i. des.
+      inv STEP0.
+      exploit Thread.step_future; eauto. i. des.
+
+      assert (PROMS: Local.promise_consistent e3.(Thread.local)).
+      { eapply rtc_tau_step_promise_consistent.
+        - eapply thread_steps_pred_steps. eapply STEPS1.
+        - unguard. des.
+          + inv FAILURE; inv STEP0. inv LOCAL. inv LOCAL0. ss.
+          + ii. rewrite PROMISES in PROMISE.
+            rewrite Memory.bot_get in PROMISE. clarify.
+        - eauto.
+        - eauto.
+        - eauto. }
+
+      assert (NOPROMISE: e2'.(Thread.local).(Local.promises) = Memory.bot).
+      { apply Memory.ext. i. rewrite Memory.bot_get.
+        destruct (Memory.get loc ts (Local.promises (Thread.local e2')))
+          as [[from [val released|]]|] eqn:GET; auto; cycle 1.
+        - exfalso.
+          eapply step_not_cancel_reserves_same in GET; cycle 1.
+          + econs.
+            * econs; eauto.
+            * instantiate (1:=promise_free /1\ (fun e => ~ is_cancel e)). ss.
+          + ss.
+          + des. eapply steps_not_cancel_reserves_same in GET; eauto.
+            des. eapply NORESERVES; eauto.
+        - exfalso.
+          exploit pf_step_rtc_promises_decrease.
+          { eapply STEPS0. }
+          { i. ss. des. auto. }
+          { econs; eauto. } ss. i.
+          exploit pf_step_rtc_promises_decrease.
+          { eapply STEP. }
+          { i. unfold is_cancel in *. des_ifs. }
+          { ss. eauto. }
+          ss. i. inv x2.
+          ss. unfold no_sc, no_acq_read_msgs in BREAKQ. des_ifs; try by (exfalso; eauto).
+          + apply not_and_or in BREAKQ. des; clarify.
+            apply imply_to_and in BREAKQ. des. apply NNPP in BREAKQ0.
+            unfold caps_loc in *. des. dup CAPS.
+            eapply caps_unchangable in CAPS; eauto; cycle 1.
+            { inv WF. eauto. }
+            eapply unchangable_rtc_increase in STEP; eauto. ss.
+            eapply unchangable_rtc_increase in STEPS0; eauto. inv STEPS0.
+            inv STEP1; inv STEP0. ss. inv LOCAL.
+            inv LOCAL0. clarify. eapply caps_max_view in CAPS0; eauto; cycle 1.
+            { inv WF. eauto. } des.
+            clarify. eapply PROMS in GET. ss. des_ifs. ss.
+            exploit max_full_timemap_get.
+            * apply MAX.
+            * inv WF. eapply PROMISES. eauto.
+            * i. eapply Time.lt_strorder. eapply TimeFacts.lt_le_lt; eauto.
+              etrans; eauto. eapply TimeMap.join_r.
+          + apply not_and_or in BREAKQ. des; clarify.
+            apply imply_to_and in BREAKQ. des. apply NNPP in BREAKQ0.
+            unfold caps_loc in *. des. dup CAPS.
+            eapply caps_unchangable in CAPS; eauto; cycle 1.
+            { inv WF. eauto. }
+            eapply unchangable_rtc_increase in STEP; eauto. ss.
+            eapply unchangable_rtc_increase in STEPS0; eauto. inv STEPS0.
+            inv STEP1; inv STEP0. ss. inv LOCAL.
+            eapply write_step_promise_consistent in LOCAL2; eauto.
+            inv LOCAL1. clarify. eapply caps_max_view in CAPS0; eauto; cycle 1.
+            { inv WF. eauto. } des.
+            clarify. eapply LOCAL2 in GET. ss. des_ifs. ss.
+            exploit max_full_timemap_get.
+            * apply MAX.
+            * inv WF. eapply PROMISES. eauto.
+            * i. eapply Time.lt_strorder. eapply TimeFacts.lt_le_lt; eauto.
+              etrans; eauto. eapply TimeMap.join_r.
+          + apply not_and_or in BREAKQ. des; clarify. apply NNPP in BREAKQ.
+            inv STEP1; inv STEP0. ss. inv LOCAL. inv LOCAL0. ss.
+            eapply PROMS in GET. ss. des_ifs. ss.
+            hexploit max_full_timemap_get; eauto.
+            * inv WF. eapply Memory.cap_le; eauto.
+            * i. eapply Time.lt_strorder. eapply TimeFacts.lt_le_lt; eauto.
+          + inv STEP1; inv STEP0. ss. inv LOCAL. inv LOCAL0. ss.
+            eapply PROMS in GET. ss. des_ifs. ss.
+            hexploit max_full_timemap_get; eauto.
+            * inv WF. eapply Memory.cap_le; eauto.
+            * i. eapply Time.lt_strorder. eapply TimeFacts.lt_le_lt; eauto.
+      }
+
+      destruct e2'. destruct local. ss.
+      eapply no_sc_any_sc_rtc in STEPS0; ss; cycle 1.
+      { i. des; ss. } des.
+      esplits.
+      * eapply pred_step_rtc_mon; eauto.
+        i. ss. des; auto.
+      * ss. eauto.
+  Qed.
+
+End PFCONSISTENT.
+
+
 
 Inductive added_memory_imm (tm: TimeMap.t): Memory.t -> Memory.t -> Prop :=
 | added_memory_imm_intro
@@ -60,476 +658,6 @@ Proof.
   ginduction ADDED; auto. etrans; [| apply IHADDED].
   inv H. econs; eauto. econs; eauto.
   econs. ss. eapply Time.bot_spec.
-Qed.
-
-Definition no_reserves (proms: Memory.t): Prop :=
-  forall loc to from msg (GET: Memory.get loc to proms = Some (from, msg)),
-    msg <> Message.reserve.
-
-Inductive only_reserves (proms: Memory.t): Prop :=
-| only_reserves_intro
-    (RESERVES: forall loc to from msg (GET: Memory.get loc to proms = Some (from, msg)),
-        msg = Message.reserve)
-    (FINITE: Memory.finite proms)
-.
-
-Lemma reserves_cancelable lang st vw proms0 sc mem0
-      (FINITE: Memory.finite proms0)
-      (MLE: Memory.le proms0 mem0)
-  :
-    exists proms1 mem1,
-      (<<STEPS: rtc (tau (@pred_step is_cancel lang))
-                    (Thread.mk lang st (Local.mk vw proms0) sc mem0)
-                    (Thread.mk lang st (Local.mk vw proms1) sc mem1)>>) /\
-      (<<NORESERVES: no_reserves proms1>>).
-Proof.
-  assert (exists dom,
-             (<<COMPLETE: forall loc to,
-                 (exists from, (<<GET: Memory.get loc to proms0 = Some (from, Message.reserve)>>))
-                 <-> (<<IN: List.In (loc, to) dom>>)>>)).
-  { unfold Memory.finite in *. des.
-    generalize (list_filter_exists (fun locto =>
-                                      match locto with
-                                      | (loc, to) =>
-                                        exists from, Memory.get loc to proms0 = Some (from, Message.reserve)
-                                      end) dom).
-    i. des. exists l'. split; i.
-    - eapply COMPLETE. des. esplits; eauto.
-    - eapply COMPLETE in H. des. esplits; eauto. }
-  des. ginduction dom; ss; i.
-  - exists proms0, mem0. esplits; eauto.
-    ii. clarify. eapply COMPLETE. eauto.
-  - destruct a as [loc to].
-    exploit (proj2 (COMPLETE loc to)); eauto. i. des.
-    destruct (classic (List.In (loc, to) dom)).
-    { exploit IHdom; eauto. i. split; i.
-      - des. exploit (proj1 (COMPLETE loc0 to0)); eauto.
-        i. des; clarify.
-      - exploit (proj2 (COMPLETE loc0 to0)); eauto. }
-    exploit Memory.remove_exists; eauto.
-    intros [prom1 REMOVE0].
-    exploit Memory.remove_exists.
-    { eapply MLE. eapply GET. }
-    intros [mem1 REMOVE1]. hexploit IHdom.
-    * instantiate (1:=prom1).
-      eapply Memory.remove_finite; eauto.
-    * instantiate (1:=mem1).
-      ii. erewrite Memory.remove_o in LHS; eauto. des_ifs.
-      eapply MLE in LHS. erewrite Memory.remove_o; eauto. des_ifs.
-      ss. des; clarify.
-    * i. split; i.
-      { des. erewrite Memory.remove_o in GET0; eauto. des_ifs.
-        exploit (proj1 (COMPLETE loc0 to0)); eauto. i. des; clarify. }
-      { exploit (proj2 (COMPLETE loc0 to0)); eauto. i. des; clarify.
-        exists from0. erewrite Memory.remove_o; eauto. des_ifs.
-        ss. des; clarify. }
-    * i. des. exists proms1, mem2. split; eauto.
-      econs 2.
-      { econs.
-        - instantiate (2:=ThreadEvent.promise loc from to Message.reserve Memory.op_kind_cancel).
-          econs; ss. econs. econs 1. econs; ss.
-          econs; ss. econs; eauto.
-        - eauto. }
-      { eauto. }
-Qed.
-
-Lemma promise_free_no_promise P lang (th0 th1: Thread.t lang) e
-      (NOPROMISE: th0.(Thread.local).(Local.promises) = Memory.bot)
-      (STEP: pred_step P e th0 th1)
-      (PRED: P <1= promise_free)
-  :
-    (<<STEP: pred_step P e th0 th1>>) /\
-    (<<NOPROMISE: th1.(Thread.local).(Local.promises) = Memory.bot>>).
-Proof.
-  inv STEP. dup SAT. eapply PRED in SAT. inv STEP0. inv STEP.
-  - inv STEP0. inv LOCAL. inv PROMISE; ss; des; clarify.
-    + rewrite NOPROMISE in *.
-      eapply Memory.lower_get0 in PROMISES. des.
-      erewrite Memory.bot_get in *. clarify.
-    + rewrite NOPROMISE in *.
-      eapply Memory.remove_get0 in PROMISES. des.
-      erewrite Memory.bot_get in *. clarify.
-  - inv STEP0. inv LOCAL.
-    + ss. esplits; eauto. econs; eauto. econs; eauto.
-    + ss. esplits; eauto.
-      * econs; eauto. econs; eauto.
-      * inv LOCAL0. ss.
-    + ss. esplits; eauto.
-      * econs; eauto. econs; eauto.
-      * inv LOCAL0. rewrite NOPROMISE in *.
-        exploit memory_write_bot_add; eauto. i. clarify.
-        inv WRITE. inv PROMISE. ss.
-        symmetry. eapply MemoryMerge.MemoryMerge.add_remove; eauto.
-    + ss. esplits; eauto.
-      * econs; eauto. econs; eauto.
-      * inv LOCAL1. inv LOCAL2. rewrite NOPROMISE in *.
-        exploit memory_write_bot_add; eauto. i. clarify.
-        inv WRITE. inv PROMISE. ss.
-        symmetry. eapply MemoryMerge.MemoryMerge.add_remove; eauto.
-    + ss. esplits; eauto.
-      * econs; eauto. econs; eauto.
-      * inv LOCAL0. ss.
-    + ss. esplits; eauto.
-      * econs; eauto. econs; eauto.
-      * inv LOCAL0. ss.
-    + ss. esplits; eauto.
-      * econs; eauto. econs; eauto.
-Qed.
-
-Definition caps (mem0 prom : Memory.t) (l : Loc.t) (t from : Time.t) (msg : Message.t) :=
-  forall mem1 (CAP: Memory.cap prom mem0 mem1),
-    (<<GET0: Memory.get l t mem0 = None>>) /\
-    (<<GET1: Memory.get l t mem1 = Some (from, msg)>>).
-
-Definition caps_loc (mem0 prom : Memory.t) (l : Loc.t) (t : Time.t): Prop :=
-  exists from msg, (<<CAPS: caps mem0 prom l t from msg>>).
-
-Lemma caps_unchangable mem0 prom mem1
-      (MLE: Memory.le prom mem0)
-      (CAP: Memory.cap prom mem0 mem1)
-  :
-    caps mem0 prom <4= unchangable mem1 prom.
-Proof.
-  i. exploit PR; eauto. i. des. inv CAP.
-  econs; eauto. ii. inv H.
-  destruct msg. eapply MLE in GET. clarify.
-Qed.
-
-Lemma finite_least P (l: list Time.t)
-  :
-    (exists to,
-        (<<SAT: P to>>) /\
-        (<<IN: List.In to l>>) /\
-        (<<LEAST: forall to'
-                         (IN: List.In to' l)
-                         (SAT: P to'),
-            Time.le to to'>>)) \/
-    (<<EMPTY: forall to (IN: List.In to l), ~ P to>>).
-Proof.
-  induction l.
-  - right. ii. inv IN.
-  - destruct (classic (P a)).
-    + des.
-      * destruct (Time.le_lt_dec a to).
-        { left. exists a. esplits; ss; eauto.
-          i. des; clarify; eauto. refl. }
-        { left. exists to. esplits; ss; eauto.
-          i. des; clarify; eauto. left. eauto. }
-      * left. exists a. esplits; ss; eauto.
-        i. des; clarify.
-        { refl. }
-        { exfalso. eapply EMPTY; eauto. }
-    + des.
-      * left. esplits; ss; eauto.
-        i. des; clarify. eapply LEAST; eauto.
-      * right. ii. ss. des; clarify.
-        eapply EMPTY; eauto.
-Qed.
-
-Lemma cell_elements_least cell P
-  :
-    (exists to from msg,
-        (<<GET: Cell.get to cell = Some (from, msg)>>) /\
-        (<<SAT: P to>>) /\
-        (<<LEAST: forall to' from' msg'
-                         (GET': Cell.get to' cell = Some (from', msg'))
-                         (SAT: P to'),
-            Time.le to to'>>)) \/
-    (<<EMPTY: forall to from msg
-                     (GET: Cell.get to cell = Some (from, msg)),
-        ~ P to>>).
-Proof.
-  hexploit (Cell.finite cell). i. des.
-  hexploit (finite_least (fun to => P to /\ exists from msg, Cell.get to cell = Some (from, msg)) dom).
-  i. des.
-  - left. esplits; eauto. i.
-    dup GET'. eapply H in GET'. eauto.
-  - right. ii. dup GET. eapply H in GET0.
-    eapply EMPTY in GET0. eapply GET0.
-    esplits; eauto.
-Qed.
-
-Lemma disjoint_equivalent2 from0 to0 from1 to1
-  :
-    (<<DISJOINT: Interval.disjoint (from0, to0) (from1, to1)>>) <->
-    ((<<TS0: ~ Time.lt from0 to0>>) \/ (<<TS1: ~ Time.lt from1 to1>>) \/
-     (<<TS0: Time.le (Time.meet to0 to1) (Time.join from0 from1)>>)).
-Proof.
-  set (disjoint_equivalent from0 to0 from1 to1).
-  eapply not_iff_compat in i. split; i.
-  - des. hexploit i.
-    { ii. clarify. } i.
-    apply not_and_or in H0. des; eauto.
-    apply not_and_or in H0. des; eauto.
-    right. right. red.
-    destruct (Time.le_lt_dec (Time.meet to0 to1) (Time.join from0 from1)); eauto.
-    exfalso. eauto.
-  - destruct i. hexploit H1.
-    { ii. des; eauto. eapply Time.lt_strorder.
-      eapply TimeFacts.lt_le_lt; eauto. }
-    ii. eauto.
-Qed.
-
-Lemma or_strengthen A B
-      (OR: A \/ B)
-  :
-    (A \/ ((<<NOT: ~ A>>) /\ (<<SAT: B>>))).
-Proof.
-  destruct (classic A); eauto. des; eauto.
-Qed.
-
-Lemma memory_get_ts_strong loc to mem from msg
-      (GET: Memory.get loc to mem = Some (from, msg))
-  :
-    (from = Time.bot /\ to = Time.bot) \/
-    ((<<TS: Time.lt from to>>) /\ (<<TO: to <> Time.bot>>)).
-Proof.
-  apply Memory.get_ts in GET.
-  destruct (classic (to = Time.bot)); clarify.
-  - des; clarify; eauto.
-    exfalso. eapply Time.lt_strorder.
-    eapply TimeFacts.lt_le_lt; eauto. eapply Time.bot_spec.
-  - des; clarify. right. eauto.
-Qed.
-
-Lemma memory_get_from_inj mem loc from to0 to1 msg0 msg1
-      (GET0: Memory.get loc to0 mem = Some (from, msg0))
-      (GET1: Memory.get loc to1 mem = Some (from, msg1))
-  :
-    (<<TO: to0 = to1>>) \/
-    (((<<BOT: to0 = Time.bot>>) \/ (<<BOT: to1 = Time.bot>>)) /\ (<<BOT: from = Time.bot>>) /\
-     (<<TO: to0 <> to1>>)).
-Proof.
-  exploit Memory.get_disjoint.
-  - eapply GET0.
-  - eapply GET1.
-  - i. des; clarify; eauto.
-    eapply memory_get_ts_strong in GET0.
-    eapply memory_get_ts_strong in GET1.
-    des; clarify; eauto.
-    { right. esplits; eauto. }
-    { right. esplits; eauto. }
-    exfalso. eapply x0.
-    + instantiate (1:=Time.meet to0 to1). econs; ss; eauto.
-      * unfold Time.meet. des_ifs.
-      * eapply Time.meet_l.
-    + econs; ss; eauto.
-      * unfold Time.meet. des_ifs.
-      * eapply Time.meet_r.
-Qed.
-
-
-Lemma memory_get_to_mon mem loc from0 from1 to0 to1 msg0 msg1
-      (GET0: Memory.get loc to0 mem = Some (from0, msg0))
-      (GET1: Memory.get loc to1 mem = Some (from1, msg1))
-      (TO: Time.lt from0 from1)
-  :
-    Time.lt to0 to1.
-Proof.
-  exploit Memory.get_disjoint.
-  - eapply GET0.
-  - eapply GET1.
-  - i. des; clarify.
-    + exfalso. eapply Time.lt_strorder. eauto.
-    + dup GET0. dup GET1.
-      eapply memory_get_ts_strong in GET0.
-      eapply memory_get_ts_strong in GET1.
-      des; clarify.
-      * exfalso. eapply Time.lt_strorder.
-        eapply TimeFacts.lt_le_lt; eauto. eapply Time.bot_spec.
-      * hexploit (Time.bot_spec from1). i.
-        destruct H; eauto.
-      * eapply disjoint_equivalent2 in x0. des; clarify.
-        unfold Time.meet, Time.join in *. des_ifs; eauto.
-        { destruct l; eauto. destruct H; eauto. clarify.
-          exfalso. eapply Time.lt_strorder; eauto. }
-        { destruct l; eauto. destruct H; eauto. clarify.
-          exfalso. eapply Time.lt_strorder; eauto. }
-        { exfalso. eapply Time.lt_strorder.
-          eapply TimeFacts.le_lt_lt; eauto. }
-        { exfalso. eapply Time.lt_strorder.
-          eapply TimeFacts.le_lt_lt; eauto. }
-Qed.
-
-Lemma memory_get_from_mon mem loc from0 from1 to0 to1 msg0 msg1
-      (GET0: Memory.get loc to0 mem = Some (from0, msg0))
-      (GET1: Memory.get loc to1 mem = Some (from1, msg1))
-      (TO: Time.lt to0 to1)
-  :
-    (<<FROMTO: Time.le to0 from1>>) \/
-    ((<<FROM0: from0 = Time.bot>>) /\ (<<FROM1: from1 = Time.bot>>) /\ (<<TO: to0 = Time.bot>>)).
-Proof.
-  exploit Memory.get_disjoint.
-  - eapply GET0.
-  - eapply GET1.
-  - i. des; clarify.
-    + exfalso. eapply Time.lt_strorder. eauto.
-    + dup GET0. dup GET1.
-      eapply memory_get_ts_strong in GET0.
-      eapply memory_get_ts_strong in GET1.
-      des; clarify.
-      * exfalso. eapply Time.lt_strorder.
-        eapply TimeFacts.lt_le_lt; eauto. eapply Time.bot_spec.
-      * exfalso. eapply Time.lt_strorder.
-        eapply TimeFacts.lt_le_lt; eauto. eapply Time.bot_spec.
-      * left. apply Time.bot_spec.
-      * left. destruct (Time.le_lt_dec to0 from1); auto. exfalso.
-        eapply x0.
-        { instantiate (1:=to0).
-          econs; ss. refl. }
-        { econs; ss. left. auto. }
-Qed.
-
-Lemma caps_concrete_last mem0 prom mem1 tm l t from val released
-      (RESERVE: Memory.reserve_wf prom mem0)
-      (INHABITED: Memory.inhabited mem0)
-      (MAX: Memory.max_full_timemap mem0 tm)
-      (CAP: Memory.cap prom mem0 mem1)
-      (CAPS: caps mem0 prom l t from (Message.full val released))
-  :
-    from = Memory.max_ts l mem0.
-Proof.
-  exploit CAPS; eauto. i. des. inv CAP.
-  exploit COMPLETE; eauto. i. des.
-  destruct (classic (Memory.max_ts l mem0 = from)); eauto. exfalso.
-  set (@cell_elements_least
-         (mem0 l)
-         (fun to => Time.lt from to)). des.
-  + assert (TLE: Time.le from from0).
-    { dup GET. eapply Memory.get_ts in GET. des; clarify.
-      { exfalso. eapply Time.lt_strorder.
-        eapply TimeFacts.lt_le_lt; eauto. eapply Time.bot_spec. }
-      exploit memory_get_from_mon.
-      - eapply x.
-      - eapply GET2.
-      - eauto.
-      - i. des; clarify. refl. }
-    destruct TLE.
-    * exploit MIDDLE; eauto.
-      econs.
-      { eapply x. }
-      { eapply GET. }
-      { eauto. }
-      { i. destruct (Memory.get l ts mem0) eqn: GET2; auto.
-        destruct p. exfalso. dup GET2. eapply LEAST in GET2; eauto.
-        eapply Memory.get_ts in GET. des; clarify.
-        - eapply Time.lt_strorder. eapply TimeFacts.lt_le_lt.
-          eapply SAT. eapply Time.bot_spec.
-        - eapply Time.lt_strorder. eapply TimeFacts.lt_le_lt.
-          eapply GET. etrans; eauto. }
-      { i. exploit memory_get_from_inj.
-        - eapply x1.
-        - eapply GET1.
-        - i. des; clarify. eapply Time.lt_strorder; eauto. }
-    * destruct H0.
-      exploit memory_get_from_inj.
-      { eapply GET1. }
-      { eapply SOUND. eapply GET. }
-      { i. des; clarify.
-        - unfold Memory.get in GET0. clarify.
-        - eapply Time.lt_strorder; eauto. }
-  + exploit Memory.max_ts_spec.
-    { eapply x. } i. des.
-    eapply EMPTY; eauto. destruct MAX0; clarify.
-    exfalso. eauto.
-Qed.
-
-Lemma caps_max_view mem0 prom mem1 tm l t from val released
-      (RESERVE: Memory.reserve_wf prom mem0)
-      (INHABITED: Memory.inhabited mem0)
-      (MAX: Memory.max_full_timemap mem0 tm)
-      (CAP: Memory.cap prom mem0 mem1)
-      (CAPS: caps mem0 prom l t from (Message.full val released))
-  :
-    (<<FROM: from = Memory.max_ts l mem0>>) /\
-    (<<RESERVE: Memory.latest_reserve l prom mem0>>) /\
-    (<<VAL: Memory.latest_val l mem0 val >>) /\
-    (<<RELEASED: released = Some (View.mk tm tm)>>) /\
-    (<<TO: t = Time.incr (Memory.max_ts l mem0)>>).
-Proof.
-  exploit caps_concrete_last; eauto. i. clarify.
-  exploit CAPS; eauto. i. des. inv CAP.
-  exploit COMPLETE; eauto. i. des.
-  exploit Memory.latest_val_exists; eauto. i. des.
-  exploit BACK; eauto. i.
-  exploit memory_get_from_inj.
-  { eapply x1. }
-  { eapply GET1. } i. des; clarify.
-  - esplits; eauto.
-  - exfalso. eapply Time.lt_strorder. eapply TimeFacts.lt_le_lt.
-    + eapply Time.incr_spec.
-    + erewrite BOT0. eapply Time.bot_spec.
-  - erewrite INHABITED in GET0. clarify.
-Qed.
-
-Lemma write_promises_decrease prom0 mem0 loc from to val realeased prom1 mem1 kind
-      (WRITE: Memory.write prom0 mem0 loc from to val realeased prom1 mem1 kind)
-  :
-    concrete_promised prom1 <2= concrete_promised prom0.
-Proof.
-  inv WRITE. inv PROMISE.
-  - exploit MemoryMerge.MemoryMerge.add_remove.
-    + eapply PROMISES.
-    + eapply REMOVE.
-    + i. clarify.
-  - ii. inv PR.
-    erewrite Memory.remove_o in GET; eauto. des_ifs.
-    erewrite Memory.split_o in GET; eauto. des_ifs.
-    + ss; des; clarify.
-    + ss. des; clarify. eapply Memory.split_get0 in PROMISES.
-      des. econs; eauto.
-    + eapply Memory.split_get0 in PROMISES.
-      guardH o. guardH o0. guardH o1. des. econs; eauto.
-  - ii. inv PR.
-    erewrite Memory.remove_o in GET; eauto. des_ifs.
-    erewrite Memory.lower_o in GET; eauto. des_ifs.
-    + ss; des; clarify.
-    + econs; eauto.
-  - clarify.
-Qed.
-
-Lemma pf_step_promises_decrease P lang e (th0 th1: Thread.t lang)
-      (STEP: (@pred_step P lang) e th0 th1)
-      (PRED: P <1= promise_free)
-  :
-    concrete_promised (th1.(Thread.local).(Local.promises)) <2=
-    concrete_promised (th0.(Thread.local).(Local.promises)).
-Proof.
-  i. inv STEP. eapply PRED in SAT. inv STEP0. des. inv STEP.
-  - inv STEP0. ss. inv LOCAL. ss. inv PROMISE; clarify.
-    + inv PR. erewrite Memory.lower_o in GET; eauto. des_ifs.
-      * ss; des. clarify. eapply Memory.lower_get0 in PROMISES.
-        des. econs; eauto.
-      * econs; eauto.
-    + inv PR. erewrite Memory.remove_o in GET; eauto. des_ifs.
-      econs; eauto.
-  - inv STEP0. ss. inv LOCAL; eauto.
-    + inv LOCAL0. ss.
-    + inv LOCAL0. ss. eapply write_promises_decrease; eauto.
-    + inv LOCAL1. inv LOCAL2. ss. eapply write_promises_decrease; eauto.
-    + inv LOCAL0. ss.
-    + inv LOCAL0. ss.
-Qed.
-
-Lemma pf_step_rtc_promises_decrease P lang (th0 th1: Thread.t lang)
-      (STEP: rtc (tau (@pred_step P lang)) th0 th1)
-      (PRED: P <1= promise_free)
-  :
-    concrete_promised (th1.(Thread.local).(Local.promises)) <2=
-    concrete_promised (th0.(Thread.local).(Local.promises)).
-Proof.
-  ginduction STEP; ss.
-  i. eapply IHSTEP in PR; eauto. inv H.
-  eapply pf_step_promises_decrease; eauto.
-Qed.
-
-Lemma le_inhabited mem0 mem1
-      (INHABITED: Memory.inhabited mem0)
-      (MLE: Memory.le mem0 mem1)
-  :
-    Memory.inhabited mem1.
-Proof.
-  ii. eapply MLE; eauto.
 Qed.
 
 Inductive configuration_step: forall (e:MachineEvent.t) (tid:Ident.t) (c1 c2:Configuration.t), Prop :=
@@ -558,418 +686,6 @@ Proof.
     + econs 2; eauto.
 Qed.
 
-Lemma no_sc_any_sc_rtc
-      P lang th_src th_tgt th_tgt' st st' lc lc' sc sc_src sc'
-      mem mem'
-      (STEP: rtc (tau (@pred_step P lang)) th_tgt th_tgt')
-      (TH_SRC: th_src = Thread.mk lang st lc sc_src mem)
-      (TH_TGT0: th_tgt = Thread.mk lang st lc sc mem)
-      (TH_TGT1: th_tgt' = Thread.mk lang st' lc' sc' mem')
-      (PRED: P <1= no_sc)
-  :
-    exists sc_src',
-      (<<STEP: rtc (tau (@pred_step P lang))
-                   th_src
-                   (Thread.mk lang st' lc' sc_src' mem')>>).
-Proof.
-  ginduction STEP.
-  - i. clarify. esplits; eauto.
-  - i. clarify. destruct y. destruct local, lc, lc'. ss.
-    inv H. exploit no_sc_any_sc; eauto. i. des.
-    exploit IHSTEP; eauto. i. des.
-    exists sc_src'0. esplits. econs; eauto.
-Qed.
-
-Lemma max_full_timemap_get mem tm loc to from val released
-      (MAX: Memory.max_full_timemap mem tm)
-      (GET: Memory.get loc to mem = Some (from, Message.full val released) )
-  :
-    Time.le to (tm loc).
-Proof.
-  specialize (MAX loc). inv MAX. eapply MAX0; eauto.
-Qed.
-
-Lemma unchangable_rtc_increase P lang (th0 th1: Thread.t lang)
-      (STEPS: rtc (tau (@pred_step P lang))th0 th1)
-  :
-    unchangable th0.(Thread.memory) th0.(Thread.local).(Local.promises) <4=
-    unchangable th1.(Thread.memory) th1.(Thread.local).(Local.promises).
-Proof.
-  ginduction STEPS; ss. i.
-  eapply IHSTEPS.
-  inv H. inv TSTEP. inv STEP. eapply unchangable_increase; eauto.
-Qed.
-
-Lemma promise_not_cacncel_reserves_same prom0 mem0 loc from to msg prom1 mem1 kind
-      (PROM: Memory.promise prom0 mem0 loc from to msg prom1 mem1 kind)
-      (NOTCANCEL: kind <> Memory.op_kind_cancel)
-      loc0 to0 from0
-      (GET: Memory.get loc0 to0 prom0 = Some (from0, Message.reserve))
-  :
-    exists from1,
-      Memory.get loc0 to0 prom1 = Some (from1, Message.reserve).
-Proof.
-  inv PROM.
-  - eapply Memory.add_get1 in GET; eauto.
-  - des. clarify. erewrite Memory.split_o; eauto.
-    dup PROMISES. eapply Memory.split_get0 in PROMISES0.
-    eapply split_succeed_wf in PROMISES. des. des_ifs.
-    + ss. des. clarify.
-    + ss. guardH o. des. clarify.
-      esplits; eauto.
-    + esplits; eauto.
-  - des. clarify. erewrite Memory.lower_o; eauto. des_ifs.
-    + ss. des. clarify.
-      eapply lower_succeed_wf in PROMISES. des. clarify.
-    + esplits; eauto.
-  - clarify.
-Qed.
-
-Lemma remove_not_cacncel_reserves_same prom0 loc from to val released prom1
-      (REMOVE: Memory.remove prom0 loc from to (Message.full val released) prom1)
-      loc0 to0 from0
-      (GET: Memory.get loc0 to0 prom0 = Some (from0, Message.reserve))
-  :
-    exists from1,
-      Memory.get loc0 to0 prom1 = Some (from1, Message.reserve).
-Proof.
-  dup REMOVE. eapply Memory.remove_get0 in REMOVE. des.
-  eapply Memory.remove_o in REMOVE0.
-  instantiate (1:=to0) in REMOVE0.
-  instantiate (1:=loc0) in REMOVE0. des_ifs.
-  - ss. des. clarify.
-  - esplits. etrans; eauto.
-Qed.
-
-Lemma step_not_cancel_reserves_same P lang e th0 th1
-      (STEPS: (@pred_step P lang) e th0 th1)
-      (PRED: P <1= (promise_free /1\ (fun e => ~ is_cancel e)))
-      loc to from
-      (GET: Memory.get loc to th0.(Thread.local).(Local.promises) = Some (from, Message.reserve))
-  :
-    exists from',
-      Memory.get loc to th1.(Thread.local).(Local.promises) = Some (from', Message.reserve).
-Proof.
-  inv STEPS. eapply PRED in SAT. inv STEP. inv STEP0.
-  - inv STEP. des. ss. inv LOCAL.
-    eapply promise_not_cacncel_reserves_same; eauto.
-    ii. clarify.
-  - inv STEP. inv LOCAL; ss.
-    + esplits; eauto.
-    + inv LOCAL0. esplits; eauto.
-    + inv LOCAL0. inv WRITE. ss.
-      eapply promise_not_cacncel_reserves_same in GET; cycle 1; eauto.
-      { ii. clarify. inv PROMISE. clarify. } des.
-      eapply remove_not_cacncel_reserves_same in GET; cycle 1; eauto.
-    + inv LOCAL2. inv WRITE. ss. inv LOCAL1. ss.
-      eapply promise_not_cacncel_reserves_same in GET; cycle 1; eauto.
-      { ii. clarify. inv PROMISE. clarify. } des.
-      eapply remove_not_cacncel_reserves_same in GET; cycle 1; eauto.
-    + inv LOCAL0. esplits; eauto.
-    + inv LOCAL0. esplits; eauto.
-    + inv LOCAL0. esplits; eauto.
-Qed.
-
-Lemma steps_not_cancel_reserves_same P lang th0 th1
-      (STEPS: rtc (tau (@pred_step P lang)) th0 th1)
-      (PRED: P <1= (promise_free /1\ (fun e => ~ is_cancel e)))
-      loc to from
-      (GET: Memory.get loc to th0.(Thread.local).(Local.promises) = Some (from, Message.reserve))
-  :
-    exists from',
-      Memory.get loc to th1.(Thread.local).(Local.promises) = Some (from', Message.reserve).
-Proof.
-  ginduction STEPS; i.
-  - esplits; eauto.
-  - inv H. exploit step_not_cancel_reserves_same; eauto. i. des.
-    exploit IHSTEPS; eauto.
-Qed.
-
-Lemma cancel_promises_decrease P lang e th0 th1
-      (STEP: (@pred_step P lang) e th0 th1)
-      (PRED: P <1= is_cancel)
-  :
-    Memory.le th1.(Thread.local).(Local.promises) th0.(Thread.local).(Local.promises).
-Proof.
-  inv STEP. eapply PRED in SAT. unfold is_cancel in SAT. des_ifs.
-  inv STEP0. inv STEP; inv STEP0; ss.
-  - inv LOCAL. inv PROMISE; ss.
-    ii. erewrite Memory.remove_o in LHS; eauto. des_ifs.
-  - inv LOCAL.
-Qed.
-
-Lemma cancels_promises_decrease P lang th0 th1
-      (STEP: rtc (tau (@pred_step P lang)) th0 th1)
-      (PRED: P <1= is_cancel)
-  :
-    Memory.le th1.(Thread.local).(Local.promises) th0.(Thread.local).(Local.promises).
-Proof.
-  ginduction STEP.
-  - refl.
-  - etrans; eauto. inv H.
-    eapply cancel_promises_decrease; eauto.
-Qed.
-
-Definition wf_time_evt (P: Loc.t -> Time.t -> Prop) (e: ThreadEvent.t) : Prop :=
-  match e with
-  | ThreadEvent.promise loc from to msg kind =>
-    (<<FROM: P loc from>>) /\ (<<TO: P loc to>>)
-  | ThreadEvent.write loc from to val released ordw =>
-    (<<FROM: P loc from>>) /\ (<<TO: P loc to>>)
-  | ThreadEvent.update loc from to valr valw releasedr releasedw ordr ordw =>
-    (<<TO: P loc to>>)
-  | _ => True
-  end.
-
-Lemma wf_time_evt_mon P0 P1
-      (LE: P0 <2= P1)
-  :
-    wf_time_evt P0 <1= wf_time_evt P1.
-Proof.
-  ii. unfold wf_time_evt in *. des_ifs; des; splits; eauto.
-Qed.
-
-Lemma step_times_list_exists P lang th0 th1 e
-      (STEPS: (@pred_step P lang) e th0 th1)
-  :
-    exists times,
-      (@pred_step (P /1\ wf_time_evt (fun loc to => List.In to (times loc))) lang) e th0 th1.
-Proof.
-  inv STEPS. destruct e.
-  - exists (fun l => if Loc.eq_dec l loc then
-                       [from; to] else []).
-    econs; eauto.
-    ss. splits; auto; des_ifs; ss; eauto.
-  - exists (fun _ => []). econs; eauto. ss.
-  - exists (fun _ => []). econs; eauto. ss.
-  - exists (fun l => if Loc.eq_dec l loc then
-                       [from; to] else []).
-    econs; eauto.
-    ss. splits; auto; des_ifs; ss; eauto.
-  - exists (fun l => if Loc.eq_dec l loc then
-                       [tsw] else []).
-    econs; eauto.
-    ss. splits; auto; des_ifs; ss; eauto.
-  - exists (fun _ => []). econs; eauto. ss.
-  - exists (fun _ => []). econs; eauto. ss.
-  - exists (fun _ => []). econs; eauto. ss.
-Qed.
-
-Lemma times_list_exists P lang th0 th1
-      (STEPS: rtc (tau (@pred_step P lang)) th0 th1)
-  :
-    exists times,
-      rtc (tau (@pred_step (P /1\ wf_time_evt (fun loc to => List.In to (times loc))) lang)) th0 th1.
-Proof.
-  ginduction STEPS.
-  - exists (fun _ => []). refl.
-  - dup H. inv H0.
-    eapply step_times_list_exists in TSTEP. des.
-    exists (fun loc => times loc ++ times0 loc). econs 2.
-    + econs; eauto. eapply pred_step_mon; eauto.
-      i. ss. des. split; auto.
-      eapply wf_time_evt_mon; eauto.
-      i. ss. eapply List.in_or_app; eauto.
-    + eapply pred_step_rtc_mon; eauto.
-      i. ss. des. split; auto.
-      eapply wf_time_evt_mon; eauto.
-      i. ss. eapply List.in_or_app; eauto.
-Qed.
-
-Definition pf_consistent_strong lang (e0:Thread.t lang): Prop :=
-  forall mem1 sc1
-         (CAP: Memory.cap e0.(Thread.local).(Local.promises) e0.(Thread.memory) mem1),
-  exists e1,
-    (<<STEPS0: rtc (tau (@pred_step is_cancel lang)) (Thread.mk _ e0.(Thread.state) e0.(Thread.local) sc1 mem1) e1>>) /\
-    (<<NORESERVE: no_reserves e1.(Thread.local).(Local.promises)>>) /\
-    exists e2,
-      (<<STEPS1: rtc (tau (@pred_step ((promise_free /1\ (fun e => ~ is_cancel e) /1\ no_acq_read_msgs (caps_loc e0.(Thread.memory) e0.(Thread.local).(Local.promises))) /1\ no_sc) lang)) e1 e2>>) /\
-      ((<<FAILURE: Local.failure_step e2.(Thread.local)>>) \/
-       (<<PROMISES: e2.(Thread.local).(Local.promises) = Memory.bot>>)).
-
-Lemma pf_consistent_pf_consistent_strong lang (th: Thread.t lang)
-      (WF: Local.wf th.(Thread.local) th.(Thread.memory))
-      (MEM: Memory.closed th.(Thread.memory))
-      (INHABITED: Memory.inhabited th.(Thread.memory))
-      (CONSISTENT: pf_consistent th)
-  :
-    pf_consistent_strong th.
-Proof.
-  ii. exploit Memory.max_full_timemap_exists; eauto. intros MAX. des.
-  ii. exploit Memory.max_full_timemap_exists.
-  { eapply le_inhabited; eauto. eapply Memory.cap_le; eauto. refl. }
-  i. des. exploit CONSISTENT; eauto. i.
-
-  assert (exists e2,
-             (<<STEPS: rtc (tau (Thread.step true))
-                           (Thread.mk _ (Thread.state th) (Thread.local th)
-                                      tm0 mem1) e2 >>) /\
-             (<<NORESERVES: no_reserves e2.(Thread.local).(Local.promises)>>) /\
-             (__guard__ ((exists e3, (<< FAILURE: Thread.step true ThreadEvent.failure e2 e3 >>)) \/
-                         (<<PROMISES: Local.promises (Thread.local e2) = Memory.bot >>)))).
-  { des.
-    - exploit Thread.rtc_tau_step_future.
-      + eapply rtc_implies; [|apply STEPS].
-        i. inv PR. econs; eauto. econs; eauto.
-      + ss. eapply Local.cap_wf; eauto.
-      + ss. eapply Memory.max_full_timemap_closed; eauto.
-      + ss. eapply Memory.cap_closed; eauto.
-      + i. des.
-        destruct e2. destruct local. inv WF2. ss.
-        exploit reserves_cancelable; eauto. i. des.
-        esplits.
-        * etrans.
-          { eapply STEPS. }
-          { eapply rtc_implies; [|apply STEPS0].
-            i. inv PR. inv TSTEP. inv STEP.
-            unfold is_cancel in SAT. des_ifs.
-            inv STEP0; inv STEP.
-            - econs; eauto. econs; eauto. econs; eauto.
-            - inv LOCAL. }
-        * ss.
-        * left. inv FAILURE; inv STEP. inv LOCAL. inv LOCAL0.
-          exists (Thread.mk _ st2 (Local.mk tview proms1) sc2 mem0).
-          ss. econs 2. econs; eauto. econs; eauto. econs; eauto.
-          eapply cancels_promises_decrease in STEPS0; auto. ss.
-          ii. eapply CONSISTENT0; eauto.
-    - unguard. esplits; eauto. rewrite PROMISES. ii.
-      rewrite Memory.bot_get in GET. clarify. }
-
-  clear x. des.
-  eapply pf_step_promise_free_step_rtc in STEPS.
-  eapply pf_steps_cancels_not_cancels in STEPS; cycle 1.
-  { ss. eapply Local.cap_wf; eauto. }
-  { ss. eapply Memory.cap_closed; eauto. }
-  { ss. eapply Memory.max_full_timemap_closed; eauto. } des.
-
-  exploit Thread.rtc_tau_step_future.
-  { eapply thread_steps_pred_steps. eapply STEPS1. }
-  { ss. eapply Local.cap_wf; eauto. }
-  { ss. eapply Memory.max_full_timemap_closed; eauto. }
-  { ss. eapply Memory.cap_closed; eauto. }
-  i. des. ss.
-
-  destruct th1. exploit no_sc_any_sc_rtc; try apply STEPS1; ss.
-  { i. unfold is_cancel in PR. des_ifs. }
-  i. des. instantiate (1:=sc1) in STEP. clear STEPS1.
-
-  eexists. splits.
-  { eapply STEP. }
-  { ss. ii. clarify.
-    eapply steps_not_cancel_reserves_same in STEPS2; eauto.
-    unguard. des.
-    - eapply NORESERVES; eauto.
-    - rewrite PROMISES in *. erewrite Memory.bot_get in STEPS2. clarify. }
-
-  eapply hold_or_not with (Q := no_acq_read_msgs (caps_loc (Thread.memory th) (Local.promises (Thread.local th))) /1\ no_sc) in STEPS2. des.
-
-  - destruct e2. ss.
-    exploit no_sc_any_sc_rtc; try eapply HOLD; eauto.
-    { ss. i. des. auto. } i. des.
-    esplits.
-    + eapply pred_step_rtc_mon; try eapply STEP0.
-      i. ss. des. splits; eauto.
-    + ss. unguard. des.
-      * left. ss. inv FAILURE; inv STEP1. inv LOCAL. eauto.
-      * right. esplits; eauto.
-
-  - exploit Thread.rtc_tau_step_future.
-    { eapply thread_steps_pred_steps. eapply STEPS0. }
-    { ss. }
-    { ss. }
-    { ss. } i. des.
-    inv STEP0.
-    exploit Thread.step_future; eauto. i. des.
-
-    assert (PROMS: Local.promise_consistent e3.(Thread.local)).
-    { eapply rtc_tau_step_promise_consistent.
-      - eapply thread_steps_pred_steps. eapply STEPS1.
-      - unguard. des.
-        + inv FAILURE; inv STEP0. inv LOCAL. inv LOCAL0. ss.
-        + ii. rewrite PROMISES in PROMISE.
-          rewrite Memory.bot_get in PROMISE. clarify.
-      - eauto.
-      - eauto.
-      - eauto. }
-
-    assert (NOPROMISE: e2'.(Thread.local).(Local.promises) = Memory.bot).
-    { apply Memory.ext. i. rewrite Memory.bot_get.
-      destruct (Memory.get loc ts (Local.promises (Thread.local e2')))
-        as [[from [val released|]]|] eqn:GET; auto; cycle 1.
-      - exfalso.
-        eapply step_not_cancel_reserves_same in GET; cycle 1.
-        + econs.
-          * econs; eauto.
-          * instantiate (1:=promise_free /1\ (fun e => ~ is_cancel e)). ss.
-        + ss.
-        + des. eapply steps_not_cancel_reserves_same in GET; eauto.
-          des. eapply NORESERVES; eauto.
-      - exfalso.
-        exploit pf_step_rtc_promises_decrease.
-        { eapply STEPS0. }
-        { i. ss. des. auto. }
-        { econs; eauto. } ss. i.
-        exploit pf_step_rtc_promises_decrease.
-        { eapply STEP. }
-        { i. unfold is_cancel in *. des_ifs. }
-        { ss. eauto. }
-        ss. i. inv x2.
-        ss. unfold no_sc, no_acq_read_msgs in BREAKQ. des_ifs; try by (exfalso; eauto).
-        + apply not_and_or in BREAKQ. des; clarify.
-          apply imply_to_and in BREAKQ. des. apply NNPP in BREAKQ0.
-          unfold caps_loc in *. des. dup CAPS.
-          eapply caps_unchangable in CAPS; eauto; cycle 1.
-          { inv WF. eauto. }
-          eapply unchangable_rtc_increase in STEP; eauto. ss.
-          eapply unchangable_rtc_increase in STEPS0; eauto. inv STEPS0.
-          inv STEP1; inv STEP0. ss. inv LOCAL.
-          inv LOCAL0. clarify. eapply caps_max_view in CAPS0; eauto; cycle 1.
-          { inv WF. eauto. } des.
-          clarify. eapply PROMS in GET. ss. des_ifs. ss.
-          exploit max_full_timemap_get.
-          * apply MAX.
-          * inv WF. eapply PROMISES. eauto.
-          * i. eapply Time.lt_strorder. eapply TimeFacts.lt_le_lt; eauto.
-            etrans; eauto. eapply TimeMap.join_r.
-        + apply not_and_or in BREAKQ. des; clarify.
-          apply imply_to_and in BREAKQ. des. apply NNPP in BREAKQ0.
-          unfold caps_loc in *. des. dup CAPS.
-          eapply caps_unchangable in CAPS; eauto; cycle 1.
-          { inv WF. eauto. }
-          eapply unchangable_rtc_increase in STEP; eauto. ss.
-          eapply unchangable_rtc_increase in STEPS0; eauto. inv STEPS0.
-          inv STEP1; inv STEP0. ss. inv LOCAL.
-          eapply write_step_promise_consistent in LOCAL2; eauto.
-          inv LOCAL1. clarify. eapply caps_max_view in CAPS0; eauto; cycle 1.
-          { inv WF. eauto. } des.
-          clarify. eapply LOCAL2 in GET. ss. des_ifs. ss.
-          exploit max_full_timemap_get.
-          * apply MAX.
-          * inv WF. eapply PROMISES. eauto.
-          * i. eapply Time.lt_strorder. eapply TimeFacts.lt_le_lt; eauto.
-            etrans; eauto. eapply TimeMap.join_r.
-        + apply not_and_or in BREAKQ. des; clarify. apply NNPP in BREAKQ.
-          inv STEP1; inv STEP0. ss. inv LOCAL. inv LOCAL0. ss.
-          eapply PROMS in GET. ss. des_ifs. ss.
-          hexploit max_full_timemap_get; eauto.
-          * inv WF. eapply Memory.cap_le; eauto.
-          * i. eapply Time.lt_strorder. eapply TimeFacts.lt_le_lt; eauto.
-        + inv STEP1; inv STEP0. ss. inv LOCAL. inv LOCAL0. ss.
-          eapply PROMS in GET. ss. des_ifs. ss.
-          hexploit max_full_timemap_get; eauto.
-          * inv WF. eapply Memory.cap_le; eauto.
-          * i. eapply Time.lt_strorder. eapply TimeFacts.lt_le_lt; eauto.
-    }
-
-    destruct e2'. destruct local. ss.
-    eapply no_sc_any_sc_rtc in STEPS0; ss; cycle 1.
-    { i. des; ss. } des.
-    esplits.
-    * eapply pred_step_rtc_mon; eauto.
-      i. ss. des; auto.
-    * ss. eauto.
-Qed.
-
 Lemma progressable_in_added_rtc
       lang st lc sc0 sc1 m0 m1 tm
       (CONSISTENT: Thread.consistent (Thread.mk lang st lc sc0 m0))
@@ -982,23 +698,3 @@ Lemma progressable_in_added_rtc
       (<<PROMISES: Local.promises (Thread.local e2) = Memory.bot>>).
 Proof.
 Admitted.
-
-Inductive diff_after_promises (prom mem0 mem1: Memory.t)
-          (caps: Loc.t -> Time.t -> Time.t -> Message.t -> Prop): Prop :=
-| diff_after_promises_intro
-    (MLE: Memory.le mem0 mem1)
-    (DIFF: forall loc to from msg
-                  (GET: Memory.get loc to mem1 = Some (from, msg))
-                  (NONE: Memory.get loc to mem0 = None),
-        (<<CAP: caps loc to from msg>>) /\
-        (exists from' to' val released,
-            (<<PROM: Memory.get loc to' prom = Some (from', Message.full val released)>>)) /\
-        (<<AFTER: forall from' to' val released
-                         (PROM: Memory.get loc to' prom = Some (from', Message.full val released)),
-            (<<TLE: Time.le to' from>>) >>))
-.
-
-
-(* Inductive my_caps (mem0 prom : Memory.t) (l : Loc.t) (t from : Time.t) (msg : Message.t) := *)
-(*   (<<CAPS: caps mem0 prom l t from msg>>) /\ *)
-(*   (<< *)
