src/drf/DRF_PF.v
@@ -397,11 +397,230 @@ Section FORGETMEMORY.
     - erewrite COMPLETE; auto. erewrite COMPLETE0; auto.
   Qed.
 
+  Lemma disjoint_equivalent from0 to0 from1 to1
+    :
+      (<<INTERSECT: ~ Interval.disjoint (from0, to0) (from1, to1)>>) <->
+      ((<<TS0: Time.lt from0 to0>>) /\ (<<TS1: Time.lt from1 to1>>) /\
+       (<<TS0: Time.lt (Time.join from0 from1) (Time.meet to0 to1)>>)).
+  Proof.
+    split; i. des.
+    - unfold Interval.disjoint in H.
+      eapply not_all_ex_not in H. des.
+      dup H. eapply not_imply_elim in H. eapply not_imply_elim2 in H0.
+      apply NNPP in H0.
+      destruct H. destruct H0. ss. splits.
+      + eapply TimeFacts.lt_le_lt; eauto.
+      + eapply TimeFacts.lt_le_lt; eauto.
+      + unfold Time.join, Time.meet. des_ifs.
+        * eapply TimeFacts.lt_le_lt; eauto.
+        * eapply TimeFacts.lt_le_lt; eauto.
+        * eapply TimeFacts.lt_le_lt; eauto.
+        * eapply TimeFacts.lt_le_lt; eauto.
+    - des. ii. eapply H.
+      + instantiate (1:=Time.meet to0 to1). econs; ss.
+        * unfold Time.join, Time.meet in *. des_ifs.
+          eapply TimeFacts.le_lt_lt; eauto.
+        * eapply Time.meet_l.
+      + econs; ss.
+        * unfold Time.join, Time.meet in *. des_ifs.
+          etrans; eauto.
+        * eapply Time.meet_r.
+  Qed.
+
+  Lemma or_strengthen A B
+        (OR: A \/ B)
+    :
+      (A \/ ((<<NOT: ~ A>>) /\ (<<SAT: B>>))).
+  Proof.
+    destruct (classic A); eauto. des; eauto.
+  Qed.
+
+  Lemma memory_get_ts_strong loc to mem from msg
+        (GET: Memory.get loc to mem = Some (from, msg))
+    :
+      (from = Time.bot /\ to = Time.bot) \/
+      ((<<TS: Time.lt from to>>) /\ (<<TO: to <> Time.bot>>)).
+  Proof.
+    apply Memory.get_ts in GET.
+    destruct (classic (to = Time.bot)); clarify.
+    - des; clarify; eauto.
+      exfalso. eapply Time.lt_strorder.
+      eapply TimeFacts.lt_le_lt; eauto. eapply Time.bot_spec.
+    - des; clarify. right. eauto.
+  Qed.
+
+  Lemma memory_get_from_inj mem loc from to0 to1 msg0 msg1
+        (GET0: Memory.get loc to0 mem = Some (from, msg0))
+        (GET1: Memory.get loc to1 mem = Some (from, msg1))
+    :
+      (<<TO: to0 = to1>>) \/
+      (((<<BOT: to0 = Time.bot>>) \/ (<<BOT: to1 = Time.bot>>)) /\ (<<BOT: from = Time.bot>>) /\
+       (<<TO: to0 <> to1>>)).
+  Proof.
+    exploit Memory.get_disjoint.
+    - eapply GET0.
+    - eapply GET1.
+    - i. des; clarify; eauto.
+      eapply memory_get_ts_strong in GET0.
+      eapply memory_get_ts_strong in GET1.
+      des; clarify; eauto.
+      { right. esplits; eauto. }
+      { right. esplits; eauto. }
+      exfalso. eapply x0.
+      + instantiate (1:=Time.meet to0 to1). econs; ss; eauto.
+        * unfold Time.meet. des_ifs.
+        * eapply Time.meet_l.
+      + econs; ss; eauto.
+        * unfold Time.meet. des_ifs.
+        * eapply Time.meet_r.
+  Qed.
+
+  Lemma disjoint_equivalent2 from0 to0 from1 to1
+    :
+      (<<DISJOINT: Interval.disjoint (from0, to0) (from1, to1)>>) <->
+      ((<<TS0: ~ Time.lt from0 to0>>) \/ (<<TS1: ~ Time.lt from1 to1>>) \/
+       (<<TS0: Time.le (Time.meet to0 to1) (Time.join from0 from1)>>)).
+  Proof.
+    set (disjoint_equivalent from0 to0 from1 to1).
+    eapply not_iff_compat in i. split; i.
+    - des. hexploit i.
+      { ii. clarify. } i.
+      apply not_and_or in H0. des; eauto.
+      apply not_and_or in H0. des; eauto.
+      right. right. red.
+      destruct (Time.le_lt_dec (Time.meet to0 to1) (Time.join from0 from1)); eauto.
+      exfalso. eauto.
+    - destruct i. hexploit H1.
+      { ii. des; eauto. eapply Time.lt_strorder.
+        eapply TimeFacts.lt_le_lt; eauto. }
+      ii. eauto.
+  Qed.
+
+  Lemma memory_get_to_mon mem loc from0 from1 to0 to1 msg0 msg1
+        (GET0: Memory.get loc to0 mem = Some (from0, msg0))
+        (GET1: Memory.get loc to1 mem = Some (from1, msg1))
+        (TO: Time.lt from0 from1)
+    :
+      Time.lt to0 to1.
+  Proof.
+    exploit Memory.get_disjoint.
+    - eapply GET0.
+    - eapply GET1.
+    - i. des; clarify.
+      + exfalso. eapply Time.lt_strorder. eauto.
+      + dup GET0. dup GET1.
+        eapply memory_get_ts_strong in GET0.
+        eapply memory_get_ts_strong in GET1.
+        des; clarify.
+        * exfalso. eapply Time.lt_strorder.
+          eapply TimeFacts.lt_le_lt; eauto. eapply Time.bot_spec.
+        * hexploit (Time.bot_spec from1). i.
+          destruct H; eauto.
+        * eapply disjoint_equivalent2 in x0. des; clarify.
+          unfold Time.meet, Time.join in *. des_ifs; eauto.
+          { destruct l; eauto. destruct H; eauto. clarify.
+            exfalso. eapply Time.lt_strorder; eauto. }
+          { destruct l; eauto. destruct H; eauto. clarify.
+            exfalso. eapply Time.lt_strorder; eauto. }
+          { exfalso. eapply Time.lt_strorder.
+            eapply TimeFacts.le_lt_lt; eauto. }
+          { exfalso. eapply Time.lt_strorder.
+            eapply TimeFacts.le_lt_lt; eauto. }
+  Qed.
+
+  Lemma memory_get_from_mon mem loc from0 from1 to0 to1 msg0 msg1
+        (GET0: Memory.get loc to0 mem = Some (from0, msg0))
+        (GET1: Memory.get loc to1 mem = Some (from1, msg1))
+        (TO: Time.lt to0 to1)
+    :
+      (<<FROMTO: Time.le to0 from1>>) \/
+      ((<<FROM0: from0 = Time.bot>>) /\ (<<FROM1: from1 = Time.bot>>) /\ (<<TO: to0 = Time.bot>>)).
+  Proof.
+    exploit Memory.get_disjoint.
+    - eapply GET0.
+    - eapply GET1.
+    - i. des; clarify.
+      + exfalso. eapply Time.lt_strorder. eauto.
+      + dup GET0. dup GET1.
+        eapply memory_get_ts_strong in GET0.
+        eapply memory_get_ts_strong in GET1.
+        des; clarify.
+        * exfalso. eapply Time.lt_strorder.
+          eapply TimeFacts.lt_le_lt; eauto. eapply Time.bot_spec.
+        * exfalso. eapply Time.lt_strorder.
+          eapply TimeFacts.lt_le_lt; eauto. eapply Time.bot_spec.
+        * left. apply Time.bot_spec.
+        * left. destruct (Time.le_lt_dec to0 from1); auto. exfalso.
+          eapply x0.
+          { instantiate (1:=to0).
+            econs; ss. refl. }
+          { econs; ss. left. auto. }
+  Qed.
+
+  Lemma max_full_timemap_get mem tm loc to from val released
+        (MAX: Memory.max_full_timemap mem tm)
+        (GET: Memory.get loc to mem = Some (from, Message.full val released))
+    :
+      Time.le to (tm loc).
+  Proof.
+    specialize (MAX loc). inv MAX. eapply MAX0; eauto.
+  Qed.
+
+  Lemma le_inhabited mem0 mem1
+        (INHABITED: Memory.inhabited mem0)
+        (MLE: Memory.le mem0 mem1)
+    :
+      Memory.inhabited mem1.
+  Proof.
+    ii. eapply MLE; eauto.
+  Qed.
+
 End FORGETMEMORY.
 
 
-
 Section MEMORYLEMMAS.
+
+  Lemma remove_le mem0 loc from to msg mem1
+        (REMOVE: Memory.remove mem0 loc from to msg mem1)
+  :
+    Memory.le mem1 mem0.
+  Proof.
+    ii. erewrite Memory.remove_o in LHS; eauto. des_ifs.
+  Qed.
+
+  Lemma step_promises_le lang (th0 th1: Thread.t lang) tf e
+        (MLE: Memory.le th0.(Thread.local).(Local.promises) th0.(Thread.memory))
+        (STEP: Thread.step tf e th0 th1)
+  :
+    Memory.le th1.(Thread.local).(Local.promises) th1.(Thread.memory).
+  Proof.
+    inv STEP.
+    - inv STEP0. inv LOCAL. ss.
+      eapply Memory.promise_le; eauto.
+    - inv STEP0. inv LOCAL; ss.
+      + inv LOCAL0; ss.
+      + inv LOCAL0. ss. inv WRITE.
+        eapply Memory.promise_le in PROMISE; eauto. red in PROMISE.
+        eapply remove_le in REMOVE.
+        etrans; eauto.
+      + inv LOCAL1. inv LOCAL2. ss. inv WRITE.
+        eapply Memory.promise_le in PROMISE; eauto. red in PROMISE.
+        eapply remove_le in REMOVE.
+        etrans; eauto.
+      + inv LOCAL0; ss.
+      + inv LOCAL0; ss.
+  Qed.
+
+  Lemma steps_promises_le P lang (th0 th1: Thread.t lang)
+        (MLE: Memory.le th0.(Thread.local).(Local.promises) th0.(Thread.memory))
+        (STEP: rtc (tau (@pred_step P lang)) th0 th1)
+  :
+    Memory.le th1.(Thread.local).(Local.promises) th1.(Thread.memory).
+  Proof.
+    ginduction STEP; ss.
+    i. eapply IHSTEP.
+    inv H. inv TSTEP. inv STEP0. eapply step_promises_le; eauto.
+  Qed.
 
   Lemma inhabited_future mem1 mem2
         (FUTURE: Memory.future mem1 mem2)
@@ -564,6 +783,61 @@ Section MEMORYLEMMAS.
     induction STEP; auto. erewrite IHSTEP; auto.
     inv H. eapply promise_bot_no_promise; eauto.
   Qed.
+
+  Lemma finite_least P (l: list Time.t)
+    :
+      (exists to,
+          (<<SAT: P to>>) /\
+          (<<IN: List.In to l>>) /\
+          (<<LEAST: forall to'
+                           (IN: List.In to' l)
+                           (SAT: P to'),
+              Time.le to to'>>)) \/
+      (<<EMPTY: forall to (IN: List.In to l), ~ P to>>).
+  Proof.
+    induction l.
+    - right. ii. inv IN.
+    - destruct (classic (P a)).
+      + des.
+        * destruct (Time.le_lt_dec a to).
+          { left. exists a. esplits; ss; eauto.
+            i. des; clarify; eauto. refl. }
+          { left. exists to. esplits; ss; eauto.
+            i. des; clarify; eauto. left. eauto. }
+        * left. exists a. esplits; ss; eauto.
+          i. des; clarify.
+          { refl. }
+          { exfalso. eapply EMPTY; eauto. }
+      + des.
+        * left. esplits; ss; eauto.
+          i. des; clarify. eapply LEAST; eauto.
+        * right. ii. ss. des; clarify.
+          eapply EMPTY; eauto.
+  Qed.
+
+  Lemma cell_elements_least cell P
+    :
+      (exists to from msg,
+          (<<GET: Cell.get to cell = Some (from, msg)>>) /\
+          (<<SAT: P to>>) /\
+          (<<LEAST: forall to' from' msg'
+                           (GET': Cell.get to' cell = Some (from', msg'))
+                           (SAT: P to'),
+              Time.le to to'>>)) \/
+      (<<EMPTY: forall to from msg
+                       (GET: Cell.get to cell = Some (from, msg)),
+          ~ P to>>).
+  Proof.
+    hexploit (Cell.finite cell). i. des.
+    hexploit (finite_least (fun to => P to /\ exists from msg, Cell.get to cell = Some (from, msg)) dom).
+    i. des.
+    - left. esplits; eauto. i.
+      dup GET'. eapply H in GET'. eauto.
+    - right. ii. dup GET. eapply H in GET0.
+      eapply EMPTY in GET0. eapply GET0.
+      esplits; eauto.
+  Qed.
+
 
 End MEMORYLEMMAS.
 
@@ -759,6 +1033,28 @@ Section NOSC.
         econs; eauto. econs; eauto. ss. f_equal.
         unfold TView.write_fence_tview. ss. des_ifs.
       + esplits. econs; eauto. econs; eauto. econs 2; eauto. econs; eauto.
+  Qed.
+
+  Lemma no_sc_any_sc_rtc
+        P lang th_src th_tgt th_tgt' st st' lc lc' sc sc_src sc'
+        mem mem'
+        (STEP: rtc (tau (@pred_step P lang)) th_tgt th_tgt')
+        (TH_SRC: th_src = Thread.mk lang st lc sc_src mem)
+        (TH_TGT0: th_tgt = Thread.mk lang st lc sc mem)
+        (TH_TGT1: th_tgt' = Thread.mk lang st' lc' sc' mem')
+        (PRED: P <1= no_sc)
+    :
+      exists sc_src',
+        (<<STEP: rtc (tau (@pred_step P lang))
+                     th_src
+                     (Thread.mk lang st' lc' sc_src' mem')>>).
+  Proof.
+    ginduction STEP.
+    - i. clarify. esplits; eauto.
+    - i. clarify. destruct y. destruct local, lc, lc'. ss.
+      inv H. exploit no_sc_any_sc; eauto. i. des.
+      exploit IHSTEP; eauto. i. des.
+      exists sc_src'0. esplits. econs; eauto.
   Qed.
 
   (* TODO: unused *)
@@ -1127,6 +1423,17 @@ Section UNCHANGABLES.
         eapply unchangable_remove; eauto.
   Qed.
 
+  Lemma unchangable_rtc_increase P lang (th0 th1: Thread.t lang)
+        (STEPS: rtc (tau (@pred_step P lang))th0 th1)
+    :
+      unchangable th0.(Thread.memory) th0.(Thread.local).(Local.promises) <4=
+      unchangable th1.(Thread.memory) th1.(Thread.local).(Local.promises).
+  Proof.
+    ginduction STEPS; ss. i.
+    eapply IHSTEPS.
+    inv H. inv TSTEP. inv STEP. eapply unchangable_increase; eauto.
+  Qed.
+
   Lemma other_promise_unchangable c tid1 tid2 st1 st2 lc1 lc2
         (CWF: Configuration.wf c)
         (TID1: IdentMap.find tid1 c.(Configuration.threads) = Some (st1, lc1))
@@ -1172,186 +1479,129 @@ Section UNCHANGABLES.
     - eapply Memory.remove_get0 in PROMISES. des. econs; eauto.
   Qed.
 
-(*   Lemma step_promise_not_in_other_spaces *)
-(*         promises1 mem1 loc from1 to1 msg promises3 mem2 kind *)
-(*         (PROMISE: Memory.promise promises1 mem1 loc from1 to1 msg promises3 mem2 kind) *)
-(*         t *)
-(*         (IN: Interval.mem (from1, to1) t) *)
-(*     : *)
-(*       ~ unwritable mem1 promises1 loc t. *)
-(*   Proof. *)
-(*     ii. inv H. inv UNCH. inv PROMISE. *)
-(*     - dup GET. eapply Memory.add_get1 in GET; eauto. *)
-(*       eapply Memory.add_get0 in MEM. des. *)
-(*       exploit Memory.get_disjoint. *)
-(*       + eapply GET. *)
-(*       + eapply GET2. *)
-(*       + i. des; clarify. eauto. *)
-(*   Admitted. *)
+  Definition unwritable2 (mem prom: Memory.t) (l: Loc.t) (t: Time.t) :=
+    (<<COV: covered l t mem>>) /\
+    (<<NCOV: ~ covered l t prom>>).
 
-(*   Lemma step_promise_not_in lang (th_tgt th_tgt': Thread.t lang) e_tgt pf *)
-(*         (STEP: Thread.step pf e_tgt th_tgt th_tgt') *)
-(*     : *)
-(*       (<<WRITE: write_not_in (unwritable th_tgt.(Thread.memory) th_tgt.(Thread.local).(Local.promises)) *)
-(*                              e_tgt>>) /\ *)
-(*       (<<PROMISE: promise_not_in (unwritable th_tgt.(Thread.memory) th_tgt.(Thread.local).(Local.promises)) *)
-(*                                  e_tgt>>) *)
-(*   . *)
-(*   Proof. *)
-(*     inv STEP. *)
-(*     - inv STEP0; ss. splits; auto. *)
-(*       ii. inv LOCAL. eapply step_promise_not_in_other_spaces; eauto. *)
-(*     - inv STEP0; ss. inv LOCAL; ss. *)
-(*       + split; auto. inv LOCAL0. inv WRITE. ii. *)
-(*         exploit step_promise_not_in_other_spaces; eauto. *)
-(*       + split; auto. inv LOCAL1. inv LOCAL2. ss. inv WRITE. ii. *)
-(*         exploit step_promise_not_in_other_spaces; eauto. *)
-(*   Qed. *)
+  Lemma unwritable_eq mem prom
+        (MLE: Memory.le prom mem)
+        l t
+    :
+      unwritable mem prom l t <-> unwritable2 mem prom l t.
+  Proof.
+    split; i.
+    - inv H. inv UNCH. econs.
+      + econs; eauto.
+      + ii. eapply NPROM. inv H.
+        exploit Memory.get_disjoint.
+        { eapply MLE. eapply GET0. }
+        { eapply GET. }
+        i. des; clarify.
+        * econs; eauto.
+        * exfalso. eapply x0; eauto.
+    - inv H. inv H0. econs; eauto. econs; eauto.
+      ii. inv H. destruct msg0. eapply H1.
+      econs; eauto. eapply MLE in GET0. clarify.
+  Qed.
 
-(*   Lemma step_wirte_not_in_write promises1 mem1 loc from1 to1 msg promises3 mem2 kind *)
-(*         (WRITE: Memory.promise promises1 mem1 loc from1 to1 msg promises3 mem2 kind) *)
-(*         t *)
-(*         (IN: Interval.mem (from1, to1) t) *)
-(*     : *)
-(*       ~ unwritable mem1 promises1 loc t. *)
-(*   Proof. *)
-(*   Admitted. *)
+  Lemma step_write_not_in_write promises1 mem1 loc from1 to1 val released promises3 mem2 kind
+        (MLE: Memory.le promises1 mem1)
+        (WRITE: Memory.write promises1 mem1 loc from1 to1 val released promises3 mem2 kind)
+        t
+        (IN: Interval.mem (from1, to1) t)
+    :
+      ~ unwritable mem1 promises1 loc t.
+  Proof.
+    rewrite unwritable_eq; auto.
+    unfold unwritable2. inv WRITE. apply or_not_and. inv PROMISE.
+    - left. ii. inv H. dup GET. eapply Memory.add_get1 in GET; eauto.
+      eapply Memory.add_get0 in MEM. des.
+      exploit Memory.get_disjoint.
+      + eapply GET.
+      + eapply GET2.
+      + i. des; clarify. eauto.
+    - right. eapply Memory.split_get0 in PROMISES. des. ii. apply H.
+      econs; eauto. inv IN. econs; ss; eauto. etrans; eauto.
+      inv MEM. inv SPLIT. left. eauto.
+    - right. eapply Memory.lower_get0 in PROMISES. des. ii. apply H.
+      econs; eauto.
+    - right. eapply Memory.remove_get0 in PROMISES. des. ii. apply H.
+      econs; eauto.
+  Qed.
 
-(*   (*   ii. inv H. inv UNCH. inv WRITE. inv UNCH. inv PROMISE. *) *)
-(*   (*   - dup GET. eapply Memory.add_get1 in GET; eauto. *) *)
-(*   (*     eapply Memory.add_get0 in MEM. des. *) *)
-(*   (*     exploit Memory.get_disjoint. *) *)
-(*   (*     + eapply GET. *) *)
-(*   (*     + eapply GET2. *) *)
-(*   (*     + i. des; clarify. eauto. *) *)
-(*   (*   - eapply Memory.split_get0 in PROMISES. des. eapply NPROM. *) *)
-(*   (*     admit. *) *)
-(*   (*   - eapply Memory.lower_get0 in PROMISES. des. eapply NPROM. *) *)
-(*   (*     econs; eauto. *) *)
-(*   (* Qed. *) *)
+  Lemma step_write_not_in lang (th_tgt th_tgt': Thread.t lang) e_tgt pf
+        (MLE: Memory.le th_tgt.(Thread.local).(Local.promises) th_tgt.(Thread.memory))
+        (STEP: Thread.step pf e_tgt th_tgt th_tgt')
+    :
+      write_not_in (unwritable th_tgt.(Thread.memory) th_tgt.(Thread.local).(Local.promises))
+                   e_tgt.
+  Proof.
+    inv STEP.
+    - inv STEP0; ss.
+    - inv STEP0; ss. inv LOCAL; ss.
+      + inv LOCAL0. ii. exploit step_write_not_in_write; eauto.
+      + inv LOCAL1. inv LOCAL2. ss. ii. exploit step_write_not_in_write; eauto.
+  Qed.
 
-(*   (* Lemma step_wirte_not_in_write promises1 mem1 loc from1 to1 val released promises3 mem2 kind *) *)
-(*   (*       (WRITE: Memory.promise promises1 mem1 loc from1 to1 val released promises3 mem2 kind) *) *)
-(*   (*       t *) *)
-(*   (*       (IN: Interval.mem (from1, to1) t) *) *)
-(*   (*   : *) *)
-(*   (*     ~ unwritable mem1 promises1 loc t. *) *)
-(*   (* Proof. *) *)
-(*   (*   ii. inv H. inv WRITE. inv UNCH. inv PROMISE. *) *)
-(*   (*   - dup GET. eapply Memory.add_get1 in GET; eauto. *) *)
-(*   (*     eapply Memory.add_get0 in MEM. des. *) *)
-(*   (*     exploit Memory.get_disjoint. *) *)
-(*   (*     + eapply GET. *) *)
-(*   (*     + eapply GET2. *) *)
-(*   (*     + i. des; clarify. eauto. *) *)
-(*   (*   - eapply Memory.split_get0 in PROMISES. des. eapply NPROM. *) *)
-(*   (*     admit. *) *)
-(*   (*   - eapply Memory.lower_get0 in PROMISES. des. eapply NPROM. *) *)
-(*   (*     econs; eauto. *) *)
-(*   (* Qed. *) *)
+  Lemma unwritable_increase pf e lang (th0 th1: Thread.t lang)
+        (STEP: Thread.step pf e th0 th1)
+    :
+      unwritable th0.(Thread.memory) th0.(Thread.local).(Local.promises) <2=
+      unwritable th1.(Thread.memory) th1.(Thread.local).(Local.promises).
+  Proof.
+    ii. inv PR.
+    eapply unchangable_increase in UNCH; eauto.
+    econs; eauto.
+  Qed.
 
-(*   (* Lemma step_wirte_not_in_write promises1 mem1 loc from1 to1 val released promises3 mem2 kind *) *)
-(*   (*       (WRITE: Memory.write promises1 mem1 loc from1 to1 val released promises3 mem2 kind) *) *)
-(*   (*       t *) *)
-(*   (*       (IN: Interval.mem (from1, to1) t) *) *)
-(*   (*   : *) *)
-(*   (*     ~ unwritable mem1 promises1 loc t. *) *)
-(*   (* Proof. *) *)
-(*   (*   ii. inv H. inv WRITE. inv UNCH. eapply NPROM. inv PROMISE. *) *)
-(*   (*   - left. ii. inv H. dup GET. eapply Memory.add_get1 in GET; eauto. *) *)
-(*   (*     eapply Memory.add_get0 in MEM. des. *) *)
-(*   (*     exploit Memory.get_disjoint. *) *)
-(*   (*     + eapply GET. *) *)
-(*   (*     + eapply GET2. *) *)
-(*   (*     + i. des; clarify. eauto. *) *)
-(*   (*   - right. eapply Memory.split_get0 in PROMISES. des. ii. apply H. *) *)
-(*   (*     econs; eauto. inv IN. econs; ss; eauto. etrans; eauto. *) *)
-(*   (*     inv MEM. inv SPLIT. left. eauto. *) *)
-(*   (*   - right. eapply Memory.lower_get0 in PROMISES. des. ii. apply H. *) *)
-(*   (*     econs; eauto. *) *)
-(*   (* Qed. *) *)
+  Lemma rtc_unwritable_increase lang (th0 th1: Thread.t lang)
+        (STEP: rtc (Thread.tau_step (lang:=lang)) th0 th1)
+    :
+      unwritable th0.(Thread.memory) th0.(Thread.local).(Local.promises) <2=
+      unwritable th1.(Thread.memory) th1.(Thread.local).(Local.promises).
+  Proof.
+    induction STEP; eauto.
+    i. inv H. inv TSTEP. eapply IHSTEP. eapply unwritable_increase; eauto.
+  Qed.
 
-(*   Lemma step_write_not_in lang (th_tgt th_tgt': Thread.t lang) e_tgt pf *)
-(*         (STEP: Thread.step pf e_tgt th_tgt th_tgt') *)
-(*     : *)
-(*       write_not_in (unwritable th_tgt.(Thread.memory) th_tgt.(Thread.local).(Local.promises)) *)
-(*                    e_tgt. *)
-(*   Proof. *)
-(*     inv STEP. *)
-(*     - inv STEP0; ss. *)
-(*     - inv STEP0; ss. inv LOCAL; ss. *)
-(*       + inv LOCAL0. ii. inv WRITE. exploit step_wirte_not_in_write; eauto. *)
-(*       + inv LOCAL1. inv LOCAL2. ss. ii. inv WRITE. exploit step_wirte_not_in_write; eauto. *)
-(*   Qed. *)
+  Lemma steps_write_not_in P lang (th_tgt th_tgt': Thread.t lang)
+        (MLE: Memory.le th_tgt.(Thread.local).(Local.promises) th_tgt.(Thread.memory))
+        (STEP: rtc (tau (@pred_step P lang)) th_tgt th_tgt')
+    :
+      rtc (tau (@pred_step (P /1\ write_not_in (unwritable th_tgt.(Thread.memory) th_tgt.(Thread.local).(Local.promises))) lang)) th_tgt th_tgt'.
+  Proof.
+    ginduction STEP.
+    - i. refl.
+    - i. inv H. inv TSTEP. econs 2.
+      + econs; eauto. econs; eauto.
+        split; auto. inv STEP0. eapply step_write_not_in; eauto.
+      + inv STEP0. exploit IHSTEP.
+        * eapply step_promises_le in MLE; eauto.
+        * i. eapply pred_step_rtc_mon; eauto.
+          i. ss. des. split; auto. eapply write_not_in_mon; eauto.
+          i. eapply unwritable_increase; eauto.
+  Qed.
 
-(*   Lemma unwritable_promise mem0 prom0 loc from to msg prom1 mem1 kind *)
-(*         (PROMISE: Memory.promise prom0 mem0 loc from to msg prom1 mem1 kind) *)
-(*     : *)
-(*       unwritable mem0 prom0 <2= unwritable mem1 prom1. *)
-(*   Proof. *)
-(*   Admitted. *)
-
-(*   (*   inv PROMISE. *) *)
-(*   (*   - ii. des. inv PR. econs. *) *)
-(*   (*     + red. erewrite add_covered; eauto. *) *)
-(*   (*     + red. erewrite add_covered; eauto. *) *)
-(*   (*       ii. des; clarify. dup MEM. eapply Memory.add_get0 in MEM. des. *) *)
-(*   (*       inv COV. exfalso. exploit Memory.get_disjoint. *) *)
-(*   (*       { eapply GET0. } *) *)
-(*   (*       { eapply Memory.add_get1; eauto. } *) *)
-(*   (*       i. des; clarify. eapply x0; eauto. *) *)
-(*   (*   - ii. des. econs. *) *)
-(*   (*     + red. erewrite split_covered; eauto. *) *)
-(*   (*     + red. erewrite split_covered; eauto. *) *)
-(*   (*   - ii. des. econs. *) *)
-(*   (*     + red. erewrite lower_covered; eauto. *) *)
-(*   (*     + red. erewrite lower_covered; eauto. *) *)
-(*   (* Qed. *) *)
-
-(*   Lemma other_promise_unchangable c tid1 tid2 st1 st2 lc1 lc2 *)
-(*         (CWF: Configuration.wf c) *)
-(*         (TID1: IdentMap.find tid1 c.(Configuration.threads) = Some (st1, lc1)) *)
-(*         (TID2: IdentMap.find tid2 c.(Configuration.threads) = Some (st2, lc2)) *)
-(*         (DIFF: tid1 <> tid2) *)
-(*         l t *)
-(*         (COV: covered l t lc2.(Local.promises)) *)
-(*     : *)
-(*       unchangable c.(Configuration.memory) lc1.(Local.promises) l t. *)
-(*   Proof. *)
-(*     inv CWF. inv WF. inv COV. destruct st1, st2. econs; eauto. *)
-(*     - exploit THREADS; try apply TID2; eauto. intros LCWF. inv LCWF. *)
-(*       econs; eauto. *)
-(*     - ii. inv H. exploit DISJOINT; eauto. intros LCDISJ. inv LCDISJ. *)
-(*       inv DISJOINT0. exploit DISJOINT1; eauto. i. des. *)
-(*       eapply x1; eauto. *)
-(*   Qed. *)
-
-(*   Lemma unchangables_remove mem prom0 loc from to msg prom1 *)
-(*         (PROMISE: Memory.remove prom0 loc from to msg prom1) *)
-(*     : *)
-(*       unchangables mem prom0 <2= unchangables mem prom1. *)
-(*   Proof. *)
-(*     unfold unchangables. ii. des. econs; eauto. *)
-(*     ii. eapply NCOV. inv H. erewrite Memory.remove_o in GET; eauto. *)
-(*     des_ifs. econs; eauto. *)
-(*   Qed. *)
-
-(*   Lemma unchangables_increase pf e lang (th0 th1: Thread.t lang) *)
-(*         (STEP: Thread.step pf e th0 th1) *)
-(*     : *)
-(*       unchangables th0.(Thread.memory) th0.(Thread.local).(Local.promises) <2= *)
-(*       unchangables th1.(Thread.memory) th1.(Thread.local).(Local.promises). *)
-(*   Proof. *)
-(*     inv STEP. *)
-(*     - inv STEP0; ss. inv LOCAL. i. *)
-(*       hexploit unchangables_promise; eauto. *)
-(*     - i. inv STEP0; ss. inv LOCAL; try inv LOCAL0; ss. *)
-(*       + inv WRITE. exploit unchangables_promise; eauto. *)
-(*         eapply unchangables_remove; eauto. *)
-(*       + inv LOCAL1. inv LOCAL2. ss. inv WRITE. *)
-(*         exploit unchangables_promise; eauto. *)
-(*         eapply unchangables_remove; eauto. *)
-(*   Qed. *)
+  Lemma other_promise_unwritable c tid1 tid2 st1 st2 lc1 lc2
+        (CWF: Configuration.wf c)
+        (TID1: IdentMap.find tid1 c.(Configuration.threads) = Some (st1, lc1))
+        (TID2: IdentMap.find tid2 c.(Configuration.threads) = Some (st2, lc2))
+        (DIFF: tid1 <> tid2)
+        l t
+        (COV: covered l t lc2.(Local.promises))
+    :
+      unwritable c.(Configuration.memory) lc1.(Local.promises) l t.
+  Proof.
+    inv CWF. inv WF. inv COV. destruct st1, st2.
+    rewrite unwritable_eq; cycle 1.
+    { exploit THREADS; try apply TID1. i. inv x1. auto. }
+    unfold unwritable2. esplits; eauto.
+    - exploit THREADS; try apply TID2; eauto. intros LCWF. inv LCWF.
+      econs; eauto.
+    - ii. inv H. exploit DISJOINT; eauto. intros LCDISJ. inv LCDISJ.
+      inv DISJOINT0. exploit DISJOINT1; eauto. i. des.
+      eapply x1; eauto.
+  Qed.
 
 End UNCHANGABLES.
 
@@ -1442,140 +1692,6 @@ Section OTHERPROMISEREMOVE.
   Qed.
 
 End OTHERPROMISEREMOVE.
-
-
-
-
-
-(* Section OTHERRESERVEREMOVE. *)
-
-(*   Lemma other_reserve_remove *)
-(*         P lang th_src th_tgt th_tgt' st st' v v' prom prom' sc sc' *)
-(*         mem_src mem_tgt mem_tgt' e_tgt others *)
-(*         (STEP: (@pred_step P lang) e_tgt th_tgt th_tgt') *)
-(*         (TH_SRC: th_src = Thread.mk lang st (Local.mk v prom) sc mem_src) *)
-(*         (TH_TGT0: th_tgt = Thread.mk lang st (Local.mk v prom) sc mem_tgt) *)
-(*         (TH_TGT1: th_tgt' = Thread.mk lang st' (Local.mk v' prom') sc' mem_tgt') *)
-(*         (MEM: forget_memory others mem_src mem_tgt) *)
-(*         (RESERVE: forall l t (OTHERS: others l t), *)
-(*             (<<RESERVE: *)
-(*     : *)
-(*       exists mem_src', *)
-(*         (<<STEP: (@pred_step *)
-(*                     (P /1\ no_promise) lang) *)
-(*                    e_tgt th_src *)
-(*                    (Thread.mk lang st' (Local.mk v' prom') sc' mem_src')>>) /\ *)
-(*         (<<MEM: forget_memory others mem_src' mem_tgt'>>). *)
-(*   Proof. *)
-(*     dup MEM. eapply forget_memory_le in MEM0. *)
-(*     clarify. inv STEP. des. inv STEP0. inv STEP. *)
-(*     { inv STEP0. ss; clarify. } *)
-(*     inv STEP0. inv LOCAL; ss. *)
-(*     - exists mem_src. esplits; eauto. econs; eauto. econs; eauto. *)
-(*       econs 2; eauto. econs; eauto. *)
-(*     - inv LOCAL0. ss. clarify. *)
-(*       exists mem_src. esplits; eauto. econs; eauto. econs; eauto. *)
-(*       econs 2; eauto. econs; eauto. econs; eauto. econs; eauto. *)
-(*       inv MEM. erewrite COMPLETE; eauto. *)
-(*     - ss. exploit other_promise_remove_write; eauto. *)
-(*       { exploit write_msg_wf; eauto. i. des. *)
-(*         eapply SAT1. econs; eauto. refl. } *)
-(*       i. des. exists mem_src'. esplits; eauto. *)
-(*       econs; eauto. econs; eauto. econs 2; eauto. econs; eauto. *)
-(*     - ss. inv LOCAL1. ss. *)
-(*       exploit other_promise_remove_write; eauto. *)
-(*       { exploit write_msg_wf; eauto. i. des. *)
-(*         eapply SAT1. econs; eauto. refl. } *)
-(*       i. des. exists mem_src'. esplits; eauto. *)
-(*       econs; eauto. econs; eauto. econs 2; eauto. econs; eauto. *)
-(*       econs; eauto. econs; eauto. inv MEM. erewrite COMPLETE; eauto. *)
-(*     - inv LOCAL0. ss. clarify. exists mem_src. esplits; eauto. *)
-(*       econs; eauto. econs; eauto. econs 2; eauto. econs; eauto. *)
-(*     - inv LOCAL0. ss. clarify. exists mem_src. esplits; eauto. *)
-(*       econs; eauto. econs; eauto. econs 2; eauto. econs; eauto. *)
-(*   Qed. *)
-
-
-(*   Lemma other_promise_remove_write v v' prom' *)
-(*         loc from to val releasedm released ord sc sc' mem_src *)
-(*         mem_tgt mem_tgt' kind others *)
-(*         (WRITE: Local.write_step *)
-(*                   (Local.mk v prom) sc mem_tgt *)
-(*                   loc from to val releasedm released ord *)
-(*                   (Local.mk v' prom') sc' mem_tgt' kind) *)
-(*         (MEM: forget_memory others mem_src mem_tgt) *)
-(*         (OTHERS: ~ others loc to) *)
-(*   : *)
-(*     exists mem_src', *)
-(*       (<<WRITE: Local.write_step *)
-(*                   (Local.mk v Memory.bot) sc mem_src *)
-(*                   loc from to val releasedm released ord *)
-(*                   (Local.mk v' Memory.bot) sc' mem_src' Memory.op_kind_add>>) /\ *)
-(*       (<<MEM: forget_memory others mem_src' mem_tgt'>>). *)
-(*   Proof. *)
-(*     exploit write_msg_wf; eauto. i. des. *)
-(*     inv WRITE. ss. clarify. exploit memory_write_bot_add; eauto. i. clarify. *)
-(*     dup WRITE0. inv WRITE0. inv PROMISE. *)
-(*     exploit write_succeed; eauto. *)
-(*     { instantiate (1:=mem_src). i. eapply forget_memory_le in MEM. *)
-(*       eapply memory_le_covered in COVER; eauto. ii. *)
-(*       exploit write_disjoint; try apply WRITE1; eauto. *)
-(*       { eapply Memory.bot_le. } *)
-(*       i. des; eauto. inv PROMISED. *)
-(*       erewrite Memory.bot_get in GET. clarify. } *)
-(*     i. des. exists mem2. econs; eauto. *)
-(*     inv MEM. inv WRITE. inv PROMISE. econs; i. *)
-(*     - erewrite (@Memory.add_o mem2); eauto. *)
-(*       erewrite (@Memory.add_o mem_tgt'); cycle 1; eauto. des_ifs. eauto. *)
-(*     - erewrite (@Memory.add_o mem2); eauto. des_ifs; eauto. *)
-(*       ss. des. clarify. *)
-(*   Qed. *)
-
-(*   Lemma other_promise_remove *)
-(*         P lang th_src th_tgt th_tgt' st st' v v' prom' sc sc' *)
-(*         mem_src mem_tgt mem_tgt' e_tgt others *)
-(*         (STEP: (@pred_step (P /1\ no_read_msgs others /1\ write_not_in others /1\ no_promise) lang) e_tgt th_tgt th_tgt') *)
-(*         (TH_SRC: th_src = Thread.mk lang st (Local.mk v Memory.bot) sc mem_src) *)
-(*         (TH_TGT0: th_tgt = Thread.mk lang st (Local.mk v Memory.bot) sc mem_tgt) *)
-(*         (TH_TGT1: th_tgt' = Thread.mk lang st' (Local.mk v' prom') sc' mem_tgt') *)
-(*         (MEM: forget_memory others mem_src mem_tgt) *)
-(*     : *)
-(*       exists mem_src', *)
-(*         (<<STEP: (@pred_step *)
-(*                     (P /1\ no_promise) lang) *)
-(*                    e_tgt th_src *)
-(*                    (Thread.mk lang st' (Local.mk v' Memory.bot) sc' mem_src')>>) /\ *)
-(*         (<<MEM: forget_memory others mem_src' mem_tgt'>>). *)
-(*   Proof. *)
-(*     dup MEM. eapply forget_memory_le in MEM0. *)
-(*     clarify. inv STEP. des. inv STEP0. inv STEP. *)
-(*     { inv STEP0. ss; clarify. } *)
-(*     inv STEP0. inv LOCAL; ss. *)
-(*     - exists mem_src. esplits; eauto. econs; eauto. econs; eauto. *)
-(*       econs 2; eauto. econs; eauto. *)
-(*     - inv LOCAL0. ss. clarify. *)
-(*       exists mem_src. esplits; eauto. econs; eauto. econs; eauto. *)
-(*       econs 2; eauto. econs; eauto. econs; eauto. econs; eauto. *)
-(*       inv MEM. erewrite COMPLETE; eauto. *)
-(*     - ss. exploit other_promise_remove_write; eauto. *)
-(*       { exploit write_msg_wf; eauto. i. des. *)
-(*         eapply SAT1. econs; eauto. refl. } *)
-(*       i. des. exists mem_src'. esplits; eauto. *)
-(*       econs; eauto. econs; eauto. econs 2; eauto. econs; eauto. *)
-(*     - ss. inv LOCAL1. ss. *)
-(*       exploit other_promise_remove_write; eauto. *)
-(*       { exploit write_msg_wf; eauto. i. des. *)
-(*         eapply SAT1. econs; eauto. refl. } *)
-(*       i. des. exists mem_src'. esplits; eauto. *)
-(*       econs; eauto. econs; eauto. econs 2; eauto. econs; eauto. *)
-(*       econs; eauto. econs; eauto. inv MEM. erewrite COMPLETE; eauto. *)
-(*     - inv LOCAL0. ss. clarify. exists mem_src. esplits; eauto. *)
-(*       econs; eauto. econs; eauto. econs 2; eauto. econs; eauto. *)
-(*     - inv LOCAL0. ss. clarify. exists mem_src. esplits; eauto. *)
-(*       econs; eauto. econs; eauto. econs 2; eauto. econs; eauto. *)
-(*   Qed. *)
-
-(* End OTHERPROMISEREMOVE. *)
 
 
 Section UNCHANGEDON.
@@ -2596,36 +2712,6 @@ Section MAPPED.
     - inv MSG. econs.
   Qed.
 
-  Lemma disjoint_equivalent from0 to0 from1 to1
-    :
-      (<<INTERSECT: ~ Interval.disjoint (from0, to0) (from1, to1)>>) <->
-      ((<<TS0: Time.lt from0 to0>>) /\ (<<TS1: Time.lt from1 to1>>) /\
-       (<<TS0: Time.lt (Time.join from0 from1) (Time.meet to0 to1)>>)).
-  Proof.
-    split; i. des.
-    - unfold Interval.disjoint in H.
-      eapply not_all_ex_not in H. des.
-      dup H. eapply not_imply_elim in H. eapply not_imply_elim2 in H0.
-      apply NNPP in H0.
-      destruct H. destruct H0. ss. splits.
-      + eapply TimeFacts.lt_le_lt; eauto.
-      + eapply TimeFacts.lt_le_lt; eauto.
-      + unfold Time.join, Time.meet. des_ifs.
-        * eapply TimeFacts.lt_le_lt; eauto.
-        * eapply TimeFacts.lt_le_lt; eauto.
-        * eapply TimeFacts.lt_le_lt; eauto.
-        * eapply TimeFacts.lt_le_lt; eauto.
-    - des. ii. eapply H.
-      + instantiate (1:=Time.meet to0 to1). econs; ss.
-        * unfold Time.join, Time.meet in *. des_ifs.
-          eapply TimeFacts.le_lt_lt; eauto.
-        * eapply Time.meet_l.
-      + econs; ss.
-        * unfold Time.join, Time.meet in *. des_ifs.
-          etrans; eauto.
-        * eapply Time.meet_r.
-  Qed.
-
   Lemma time_meet_map loc t0 t1 ft0 ft1
         (MAP0: f loc t0 ft0)
         (MAP1: f loc t1 ft1)
@@ -2936,18 +3022,29 @@ Section MAPPED.
         eapply Memory.add_get1; eauto.
   Qed.
 
+  Definition mapped_time loc fto :=
+    exists to, (<<MAPPED: f loc to fto>>).
+
   Definition wf_mappable_evt (e: ThreadEvent.t) : Prop :=
     match e with
     | ThreadEvent.promise loc from to msg kind =>
       match kind with
-      | Memory.op_kind_add => non_collapsable loc to
-      | Memory.op_kind_split _ _ => non_collapsable loc to
+      | Memory.op_kind_add =>
+        (<<FROM: mapped_time loc from>>) /\
+        (<<TO: mapped_time loc to>>) /\
+        (<<NCLPS: non_collapsable loc to>>)
+      | Memory.op_kind_split _ _ =>
+        (<<TO: mapped_time loc to>>) /\
+        (<<NCLPS: non_collapsable loc to>>)
       | _ => True
       end
     | ThreadEvent.write loc from to val released ordw =>
-      non_collapsable loc to
+      (<<FROM: mapped_time loc from>>) /\
+      (<<TO: mapped_time loc to>>) /\
+      (<<NCLPS: non_collapsable loc to>>)
     | ThreadEvent.update loc from to valr valw releasedr releasedw ordr ordw =>
-      non_collapsable loc to
+      (<<TO: mapped_time loc to>>) /\
+      (<<NCLPS: non_collapsable loc to>>)
     | _ => True
     end.
 
@@ -2956,6 +3053,7 @@ Section MAPPED.
         sc_src sc_tgt sc_tgt'
         mem_src mem_tgt mem_tgt' e_tgt
         (MAPPABLE: P <1= wf_mappable_evt)
+        (* (PRED: P <1= promise_free) *)
         (STEP: (@pred_step P lang) e_tgt th_tgt th_tgt')
         (TH_SRC: th_src = Thread.mk lang st (Local.mk v_src prom_src)
                                     sc_src mem_src)
@@ -2963,10 +3061,13 @@ Section MAPPED.
                                      sc_tgt mem_tgt)
         (TH_TGT1: th_tgt' = Thread.mk lang st' (Local.mk v_tgt' prom_tgt')
                                       sc_tgt' mem_tgt')
+
         (CLOSEDMAP0: Memory.closed_timemap sc_tgt mem_tgt)
         (CLOSED0: Memory.closed mem_tgt)
         (LCWF: Local.wf (Local.mk v_tgt prom_tgt) mem_tgt)
         (INHABITED: Memory.inhabited mem_tgt)
+
+        (TVIEW: tview_map v_src v_tgt)
         (MEM: memory_map mem_src mem_tgt)
         (PROM: promises_map prom_src prom_tgt)
         (SC: timemap_map sc_src sc_tgt)
@@ -2977,9 +3078,13 @@ Section MAPPED.
                    (Thread.mk lang st' (Local.mk v_src' prom_src') sc_src' mem_src')>>) /\
         (<<SC: timemap_map sc_src' sc_tgt'>>) /\
         (<<PROM: promises_map prom_src' prom_tgt'>>) /\
-        (<<MEM: memory_map mem_src' mem_tgt'>>).
+        (<<MEM: memory_map mem_src' mem_tgt'>>) /\
+        (<<TVIEW: tview_map v_src' v_tgt'>>) /\
+        (<<EVT: tevent_map e_src e_tgt>>)
+  .
   Proof.
   Admitted.
+
   (* Lemma remove_memory_map mem0 fmem0 loc from to msg mem1 *)
   (*       (REMOVE: Memory.remove mem0 loc from to msg mem1) *)
   (*       (MEM: memory_map mem0 fmem0) *)
@@ -3745,125 +3850,6 @@ End MAPPED.
 
 
 
-Section UNCHANGAGBLES.
-
-  Definition unchangables (mem prom: Memory.t) (l: Loc.t) (t: Time.t) :=
-    (<<COV: covered l t mem>>) /\
-    (<<NCOV: ~ covered l t prom>>).
-
-  Lemma step_wirte_not_in_write promises1 mem1 loc from1 to1 val released promises3 mem2 kind
-        (WRITE: Memory.write promises1 mem1 loc from1 to1 val released promises3 mem2 kind)
-        t
-        (IN: Interval.mem (from1, to1) t)
-    :
-      ~ unchangables mem1 promises1 loc t.
-  Proof.
-    unfold unchangables. inv WRITE. apply or_not_and. inv PROMISE.
-    - left. ii. inv H. dup GET. eapply Memory.add_get1 in GET; eauto.
-      eapply Memory.add_get0 in MEM. des.
-      exploit Memory.get_disjoint.
-      + eapply GET.
-      + eapply GET2.
-      + i. des; clarify. eauto.
-    - right. eapply Memory.split_get0 in PROMISES. des. ii. apply H.
-      econs; eauto. inv IN. econs; ss; eauto. etrans; eauto.
-      inv MEM. inv SPLIT. left. eauto.
-    - right. eapply Memory.lower_get0 in PROMISES. des. ii. apply H.
-      econs; eauto.
-    - right. eapply Memory.remove_get0 in PROMISES. des. ii. apply H.
-      econs; eauto.
-  Qed.
-
-  Lemma step_wirte_not_in lang (th_tgt th_tgt': Thread.t lang) e_tgt pf
-        (STEP: Thread.step pf e_tgt th_tgt th_tgt')
-    :
-      write_not_in (unchangables th_tgt.(Thread.memory) th_tgt.(Thread.local).(Local.promises))
-                   e_tgt.
-  Proof.
-    unfold unchangables. inv STEP.
-    - inv STEP0; ss.
-    - inv STEP0; ss. inv LOCAL; ss.
-      + inv LOCAL0. ii. exploit step_wirte_not_in_write; eauto.
-      + inv LOCAL1. inv LOCAL2. ss. ii. exploit step_wirte_not_in_write; eauto.
-  Qed.
-
-  Lemma unchangables_promise mem0 prom0 loc from to msg prom1 mem1 kind
-        (PROMISE: Memory.promise prom0 mem0 loc from to msg prom1 mem1 kind)
-    :
-      unchangables mem0 prom0 <2= unchangables mem1 prom1.
-  Proof.
-    unfold unchangables. inv PROMISE.
-    - ii. des. econs.
-      + red. erewrite add_covered; eauto.
-      + red. erewrite add_covered; eauto.
-        ii. des; clarify. dup MEM. eapply Memory.add_get0 in MEM. des.
-        inv COV. exfalso. exploit Memory.get_disjoint.
-        { eapply GET0. }
-        { eapply Memory.add_get1; eauto. }
-        i. des; clarify. eapply x0; eauto.
-    - ii. des. econs.
-      + red. erewrite split_covered; eauto.
-      + red. erewrite split_covered; eauto.
-    - ii. des. econs.
-      + red. erewrite lower_covered; eauto.
-      + red. erewrite lower_covered; eauto.
-    - ii. des. econs.
-      + red. erewrite remove_covered; eauto.
-        split; auto. apply not_and_or. ii. des. clarify.
-        apply Memory.remove_get0 in PROMISES. des.
-        apply NCOV. econs; eauto.
-      + red. erewrite remove_covered; eauto.
-        ii. eapply NCOV. des; auto.
-  Qed.
-
-  Lemma other_promise_unchangables c tid1 tid2 st1 st2 lc1 lc2
-        (CWF: Configuration.wf c)
-        (TID1: IdentMap.find tid1 c.(Configuration.threads) = Some (st1, lc1))
-        (TID2: IdentMap.find tid2 c.(Configuration.threads) = Some (st2, lc2))
-        (DIFF: tid1 <> tid2)
-        l t
-        (COV: covered l t lc2.(Local.promises))
-    :
-      unchangables c.(Configuration.memory) lc1.(Local.promises) l t.
-  Proof.
-    inv CWF. inv WF. inv COV. destruct st1, st2. econs; eauto.
-    - exploit THREADS; try apply TID2; eauto. intros LCWF. inv LCWF.
-      econs; eauto.
-    - ii. inv H. exploit DISJOINT; eauto. intros LCDISJ. inv LCDISJ.
-      inv DISJOINT0. exploit DISJOINT1; eauto. i. des.
-      eapply x1; eauto.
-  Qed.
-
-  Lemma unchangables_remove mem prom0 loc from to msg prom1
-        (PROMISE: Memory.remove prom0 loc from to msg prom1)
-    :
-      unchangables mem prom0 <2= unchangables mem prom1.
-  Proof.
-    unfold unchangables. ii. des. econs; eauto.
-    ii. eapply NCOV. inv H. erewrite Memory.remove_o in GET; eauto.
-    des_ifs. econs; eauto.
-  Qed.
-
-  Lemma unchangables_increase pf e lang (th0 th1: Thread.t lang)
-        (STEP: Thread.step pf e th0 th1)
-    :
-      unchangables th0.(Thread.memory) th0.(Thread.local).(Local.promises) <2=
-      unchangables th1.(Thread.memory) th1.(Thread.local).(Local.promises).
-  Proof.
-    inv STEP.
-    - inv STEP0; ss. inv LOCAL. i.
-      hexploit unchangables_promise; eauto.
-    - i. inv STEP0; ss. inv LOCAL; try inv LOCAL0; ss.
-      + inv WRITE. exploit unchangables_promise; eauto.
-        eapply unchangables_remove; eauto.
-      + inv LOCAL1. inv LOCAL2. ss. inv WRITE.
-        exploit unchangables_promise; eauto.
-        eapply unchangables_remove; eauto.
-  Qed.
-
-End UNCHANGAGBLES.
-
-
 Section SHORTERMEMORY.
 
   Inductive shorter_memory (mem_src mem_tgt: Memory.t): Prop :=
@@ -4006,14 +3992,6 @@ Section SHORTERMEMORY.
       + inv LOCAL0. ss. clarify. esplits; eauto. econs; eauto.
         econs; eauto. econs 2; eauto. econs; eauto.
   Qed.
-
-  Lemma step_promises_le lang (th0 th1: Thread.t lang) tf e
-        (MLE: Memory.le th0.(Thread.local).(Local.promises) th0.(Thread.memory))
-        (STEP: Thread.step tf e th0 th1)
-    :
-      Memory.le th1.(Thread.local).(Local.promises) th1.(Thread.memory).
-  Proof.
-  Admitted.
 
   (* Lemma shorter_memory_step2 *)
   (*       P lang th_src th_tgt th_tgt' st st' v v' prom prom' sc sc' *)
