src/drf/DRF_PF3.v
@@ -1,0 +1,170 @@
+Require Import Omega.
+Require Import RelationClasses.
+
+From Paco Require Import paco.
+From sflib Require Import sflib.
+
+From PromisingLib Require Import Axioms.
+From PromisingLib Require Import Basic.
+From PromisingLib Require Import DataStructure.
+Require Import Time.
+Require Import Event.
+From PromisingLib Require Import Language.
+Require Import View.
+Require Import Cell.
+Require Import Memory.
+Require Import Cover.
+Require Import TView.
+Require Import Local.
+Require Import Thread.
+Require Import Configuration.
+Require Import Progress.
+Require Import PromiseConsistent.
+From PromisingLib Require Import Loc.
+
+Require Import PF.
+Require Import Race.
+Require Import Behavior.
+Require Import SimMemory.
+Require Import yjtac.
+Require Import Program.
+Require Import Cell.
+Require Import Time.
+Require Import PredStep.
+Require Import ReorderPromises2.
+Require Import AbortProp.
+
+Require Import DRF_PF.
+
+Require Import PFConsistent.
+
+Set Implicit Arguments.
+
+
+
+(* Inductive my_caps (mem0 prom : Memory.t) (l : Loc.t) (t from : Time.t) (msg : Message.t) := *)
+(*   (<<CAPS: caps mem0 prom l t from msg>>) /\ *)
+(*   (<< *)
+
+
+Definition wf_time_evt (P: Loc.t -> Time.t -> Prop) (e: ThreadEvent.t) : Prop :=
+  match e with
+  | ThreadEvent.promise loc from to msg kind =>
+    (<<FROM: P loc from>>) /\ (<<TO: P loc to>>)
+  | ThreadEvent.write loc from to val released ordw =>
+    (<<FROM: P loc from>>) /\ (<<TO: P loc to>>)
+  | ThreadEvent.update loc from to valr valw releasedr releasedw ordr ordw =>
+    (<<TO: P loc to>>)
+  | _ => True
+  end.
+
+Lemma wf_time_evt_mon P0 P1
+      (LE: P0 <2= P1)
+  :
+    wf_time_evt P0 <1= wf_time_evt P1.
+Proof.
+  ii. unfold wf_time_evt in *. des_ifs; des; splits; eauto.
+Qed.
+
+Lemma step_times_list_exists P lang th0 th1 e
+      (STEPS: (@pred_step P lang) e th0 th1)
+  :
+    exists times,
+      (@pred_step (P /1\ wf_time_evt (fun loc to => List.In to (times loc))) lang) e th0 th1.
+Proof.
+  inv STEPS. destruct e.
+  - exists (fun l => if Loc.eq_dec l loc then
+                       [from; to] else []).
+    econs; eauto.
+    ss. splits; auto; des_ifs; ss; eauto.
+  - exists (fun _ => []). econs; eauto. ss.
+  - exists (fun _ => []). econs; eauto. ss.
+  - exists (fun l => if Loc.eq_dec l loc then
+                       [from; to] else []).
+    econs; eauto.
+    ss. splits; auto; des_ifs; ss; eauto.
+  - exists (fun l => if Loc.eq_dec l loc then
+                       [tsw] else []).
+    econs; eauto.
+    ss. splits; auto; des_ifs; ss; eauto.
+  - exists (fun _ => []). econs; eauto. ss.
+  - exists (fun _ => []). econs; eauto. ss.
+  - exists (fun _ => []). econs; eauto. ss.
+Qed.
+
+Lemma times_list_exists P lang th0 th1
+      (STEPS: rtc (tau (@pred_step P lang)) th0 th1)
+  :
+    exists times,
+      rtc (tau (@pred_step (P /1\ wf_time_evt (fun loc to => List.In to (times loc))) lang)) th0 th1.
+Proof.
+  ginduction STEPS.
+  - exists (fun _ => []). refl.
+  - dup H. inv H0.
+    eapply step_times_list_exists in TSTEP. des.
+    exists (fun loc => times loc ++ times0 loc). econs 2.
+    + econs; eauto. eapply pred_step_mon; eauto.
+      i. ss. des. split; auto.
+      eapply wf_time_evt_mon; eauto.
+      i. ss. eapply List.in_or_app; eauto.
+    + eapply pred_step_rtc_mon; eauto.
+      i. ss. des. split; auto.
+      eapply wf_time_evt_mon; eauto.
+      i. ss. eapply List.in_or_app; eauto.
+Qed.
+
+
+
+Inductive diff_after_promises (prom mem0 mem1: Memory.t)
+          (caps: Loc.t -> Time.t -> Time.t -> Message.t -> Prop): Prop :=
+| diff_after_promises_intro
+    (MLE: Memory.le mem0 mem1)
+    (DIFF: forall loc to from msg
+                  (GET: Memory.get loc to mem1 = Some (from, msg))
+                  (NONE: Memory.get loc to mem0 = None),
+        (<<CAP: caps loc to from msg>>) /\
+        (exists from' to' val released,
+            (<<PROM: Memory.get loc to' prom = Some (from', Message.full val released)>>)) /\
+        (<<AFTER: forall from' to' val released
+                         (PROM: Memory.get loc to' prom = Some (from', Message.full val released)),
+            (<<TLE: Time.le to' from>>) >>))
+.
+
+
+Lemma steps_write_not_in P lang (th0 th1: Thread.t lang)
+
+
+
+
+Lemma collapse_other_cappe
+
+Lemma
+
+Lemma my_
+
+
+
+Lemma step_wirte_not_in lang (th_tgt th_tgt': Thread.t lang) e_tgt pf
+      (STEP: Thread.step pf e_tgt th_tgt th_tgt')
+  :
+    write_not_in (unchangables th_tgt.(Thread.memory) th_tgt.(Thread.local).(Local.promises))
+                 e_tgt.
+Proof.
+  unfold unchangables. inv STEP.
+  - inv STEP0; ss.
+  - inv STEP0; ss. inv LOCAL; ss.
+    + inv LOCAL0. ii. exploit step_wirte_not_in_write; eauto.
+    + inv LOCAL1. inv LOCAL2. ss. ii. exploit step_wirte_not_in_write; eauto.
+Qed.
+
+
+Definition pf_consistent_strong lang (e0:Thread.t lcapped intrang): Prop :=
+  forall mem1 sc1
+         (CAP: Memory.cap e0.(Thread.local).(Local.promises) e0.(Thread.memory) mem1),
+  exists e1,
+    (<<STEPS0: rtc (tau (@pred_step is_cancel lang)) (Thread.mk _ e0.(Thread.state) e0.(Thread.local) sc1 mem1) e1>>) /\
+    (<<NORESERVE: no_reserves e1.(Thread.local).(Local.promises)>>) /\
+    exists e2,
+      (<<STEPS1: rtc (tau (@pred_step ((promise_free /1\ (fun e => ~ is_cancel e) /1\ no_acq_read_msgs (caps_loc e0.(Thread.memory) e0.(Thread.local).(Local.promises))) /1\ no_sc) lang)) e1 e2>>) /\
+      ((<<FAILURE: Local.failure_step e2.(Thread.local)>>) \/
+       (<<PROMISES: e2.(Thread.local).(Local.promises) = Memory.bot>>)).
